go

WeirdLogic/Example4.lean
@@ -13,10 +13,16 @@ import WeirdLogic.Hete
 import WeirdLogic.GramDisjStandard
 import WeirdLogic.WUnary
 
+import WeirdLogic.GramSeq
+import WeirdLogic.Example3_1
+import WeirdLogic.Example0
+
 open Unary prim val trm
 open ContextFreeGrammar
+-- #check Set.BijOn
+open Classical
 
-namespace WeirdLogic
+namespace WeirdLogic.Example4
 
 /- L -> S1; S2
   S1 -> trm1; S1; trm2
@@ -25,8 +31,10 @@ namespace WeirdLogic
   L = {trm1ⁿ;trm2ⁿ;(trm3|trm4) : n ≥ 0}
   context free + seq rule
 -/
+/-
 def trm1 : trm := [lang| let xx := !xl in let temp0 := xx + 1 in xl := temp0]
 def trm2 : trm := [lang| let yy := !yl in let temp1 := yy + 1 in yl := temp1]
+-/
 def trm3 : trm := [lang| let xx := !xl in let yy := !yl in let temp1 := xx + yy in xl := temp1]
 def trm4 : trm := [lang| let xx := !xl in let yy := !yl in let temp1 := xx - yy in xl := temp1]
 def r1 : ContextFreeRule trm String :=
@@ -38,7 +46,7 @@ def r1 : ContextFreeRule trm String :=
 def r2 : ContextFreeRule trm String :=
   {
     input := "S1",
-    output := [Symbol.terminal trm1, Symbol.nonterminal "S1", Symbol.terminal trm2],
+    output := [Symbol.terminal Example3.trm1, Symbol.nonterminal "S1", Symbol.terminal Example3.trm2],
   }
 
 def r3 : ContextFreeRule trm String :=
@@ -57,14 +65,14 @@ def cfg1 : ContextFreeGrammar trm :=
   {
     NT := String,
     initial := "S1",
-    rules := Finset.mk {r1, r2, r3, r4} (by unfold r1 r2 r3 r4 trm1 trm2; simp)
+    rules := Finset.mk {r1, r2, r3, r4} (by unfold r1 r2 r3 r4 Example3.trm1 Example3.trm2; simp)
   }
 
 def l1 : Language trm := cfg1.language
 
-
-lang_def' prog_c1 :=
-  fun ⸨xl: Loc⸩ ⸨yl: Loc⸩ ⸨pa:Val⸩ ⸨pb:Val⸩=>
+/-
+lang_def' prog_c1_pre :=
+  fun ⸨xl: Loc⸩ ⸨yl: Loc⸩ ⸨pa:Val⸩ =>
     for k in [0:pa] {
       let xx := !xl in
       let temp0 := xx + 1 in
@@ -74,7 +82,10 @@ lang_def' prog_c1 :=
       let yy := !yl in
       let temp1 := yy + 1 in
       yl := temp1
-    };
+    }
+
+lang_def' prog_c1_post :=
+  fun ⸨xl: Loc⸩ ⸨yl: Loc⸩ ⸨pb:Val⸩ =>
     let xx := !xl in
     let yy := !yl in
     if pb > 10 then
@@ -83,8 +94,13 @@ lang_def' prog_c1 :=
     else
       let temp1 := xx - yy in
       yl := temp1
+-/
 
-
+lang_def' prog_c1 :=
+  fun ⸨xl: Loc⸩ ⸨yl: Loc⸩ ⸨pa:Val⸩ ⸨pb:Val⸩=>
+    Example3.prog_c1(⸨xl:Loc⸩, ⸨yl:Loc⸩, pa);
+    Example0.prog_c1(⸨xl:Loc⸩, ⸨yl:Loc⸩, pb)
+/-
 def regexp_grammar : ℕ → trm → trm
   | 0, _ => trm_val val_unit
   | 1, t => t
@@ -93,42 +109,74 @@ def regexp_grammar : ℕ → trm → trm
 def cfgexp_grammar : ℕ → trm → trm → trm
   | 0, _, _ => trm_val val_unit
   | n, t1, t2 => trm_seq (regexp_grammar n t1) (regexp_grammar n t2)
+-/
 
 def orexp_grammar : Bool → trm
-  | true => trm3
-  | false => trm4
+  | true => Example0.trm1
+  | false => Example0.trm2
+
+syntax "⌜" term "⌝" : lang
+
+macro_rules
+  | `([lang| ⌜ $f:term ⌝($xs:lang,*) ])     => `(trm_call ($f) [ $[[lang|$xs:lang]],* ])
+
+def lang_sn1 i :=
+  Example3.cfgexp_grammar i Example3.trm1 Example3.trm2
+
+def lang_part1 i :=
+  [lang| ⌜ [lang| fun ⸨xl: Loc⸩ ⸨yl : Loc⸩ => { (lang_sn1 i) }] ⌝(⸨xl: Loc⸩, ⸨yl : Loc⸩) ]
+
+def lang_part2 b :=
+  [lang| ⌜ (orexp_grammar b) ⌝(⸨xl: Loc⸩, ⸨yl : Loc⸩) ]
 
 def lang_squeeze_list': Set trm :=
   {trm_seq
-    (cfgexp_grammar i trm1 trm2)
-    (orexp_grammar j)
+    (lang_part1 i)
+    (lang_part2 j)
     | (i : ℕ) (j : Bool) }
 
+def trm_seq_fst : trm → trm
+  | trm_seq t1 _ => t1
+  | _ => default_trm
+
+def trm_seq_snd : trm → trm
+  | trm_seq _ t2 => t2
+  | _ => default_trm
+
+def trm_call_fun : trm → trm
+  | trm_call t1 _ => t1
+  | _ => default_trm
+
+def trm_call_args : trm → List trm
+  | trm_call _ args => args
+  | _ => []
+
+/-
 def lang_squeeze_list: Set trm :=
   {trm_seq (cfgexp_grammar i trm1 trm2) (trm3) | i : ℕ } ∪ {trm_seq (cfgexp_grammar i trm1 trm2) (trm4) | i : ℕ }
 
 def lang_fun_set : Set trm :=
   {[lang| fun ⸨xl: Loc⸩ ⸨yl : Loc⸩ => {tt}] | tt ∈ lang_squeeze_list' }
-
-def pay_index : Set (trm × payload × payload) :=
+-/
+def pay_index : Set (trm × Example3.payload × payload) :=
   { x |
-    ∃ p1 ∈ @Set.univ payload, ∃ p2 ∈ @Set.univ payload, (default_trm,(p1,p2))=x
+    ∃ p1 ∈ @Set.univ Example3.payload, ∃ p2 ∈ @Set.univ payload, (default_trm,(p1,p2))=x
   }
 
-def lang_index : Set (trm × payload × payload ):=
-  { (l, (default_payload,default_payload)) | l ∈ lang_squeeze_list'}
-
+def lang_index : Set (trm × Example3.payload × payload ):=
+  { (l, (Example3.default_payload,default_payload)) | l ∈ lang_squeeze_list'}
+/-
 def lang_index1 : Set (trm × payload × payload ):=
   { (l, (default_payload,default_payload)) | l  ∈ {trm_seq (cfgexp_grammar i trm1 trm2) (trm3) | i : ℕ } }
 
 def lang_index2 : Set (trm × payload × payload ):=
   { (l, (default_payload,default_payload)) | l ∈ {trm_seq (cfgexp_grammar i trm1 trm2) (trm4) | i : ℕ } }
-
+/-
 lemma lang_union :
   lang_index = lang_index1 ∪ lang_index2 := by
   unfold lang_index1 lang_index2 lang_index lang_squeeze_list'
   aesop
-
+-/
 lemma lang_disjoint :
   Disjoint lang_index1 lang_index2 := by
   unfold lang_index1 lang_index2
@@ -183,181 +231,201 @@ lemma pay_disjoint :
   rw [heq] at h3
   have tmp := not_le_of_gt h1
   contradiction
-
+-/
 /-
   This is the proof for option 1
 -/
-set_option maxRecDepth 2000 in
-set_option maxHeartbeats 6400000 in
-lemma example4_spec0 (xv : ℤ) (yv : ℤ):
-  {
-    [∗ in ⟪0,pay_index⟫ ∪ ⟪1,lang_index⟫ | xl ~~> xv ∗ yl ~~> yv]
-  }
-  [0| p in pay_index => prog_c1(⸨xl : Loc⸩, ⸨yl : Loc⸩, ⟨p.val.2.1⟩, ⟨p.val.2.2⟩) ]
-  [1| l in lang_index => l.val.fst(⸨xl: Loc⸩, ⸨yl : Loc⸩)]
-  { v,
-    fun h => ∀ ll ∈ lang_index, ∃ pp ∈ pay_index , h ⟨1, ll⟩ = h ⟨0, pp⟩
-  }
-  := by
-  unfold LGTM.triple
-  unfold lang_index
-  sorry
-  -- dsimp
-  -- yin 1 : apply ywp_lemma_funs' (tfunc := fun i => i.val.1) (ts := fun (p : (trm × payload × payload)ˡ) => [xl, yl]);
-  -- simp;
-/-
-  Option 1: with SeqU rule
-  Option 2: without SeqU rule
-  This is the proof for option 2
--/
+
+attribute [-simp] Bool.exists_bool
+-- attribute [simp] trm_seq_fst trm_seq_snd trm_call_fun
+
+-- theorem exists_labType {p : ℕ → α → Prop} :
+--   (∃ (x : αˡ), p x.lab x.val) ↔ (∃ (l : ℕ) (a : α), p l a) := by
+--   constructor
+--   · rintro ⟨⟨xl, xval⟩, h⟩ ; exists xl, xval
+--   · rintro ⟨l, a, h⟩ ; exists ⟨l, a⟩
+theorem exists_labType {p : αˡ → Prop} :
+  (∃ (x : αˡ), p x) ↔ (∃ (l : ℕ) (a : α), p ⟨l, a⟩) := by
+  constructor
+  · rintro ⟨⟨xl, xval⟩, h⟩ ; exists xl, xval
+  · rintro ⟨l, a, h⟩ ; exists ⟨l, a⟩
+
+theorem forall_labType {p : αˡ → Prop} :
+  (∀ (x : αˡ), p x) ↔ (∀ (l : ℕ) (a : α), p ⟨l, a⟩) := by
+  constructor <;> aesop
+
 set_option maxRecDepth 2000 in
 set_option maxHeartbeats 6400000 in
 lemma example4_spec (xv : ℤ) (yv : ℤ):
+  let tfunc (i : trm) := [lang| fun ⸨xl: Loc⸩ ⸨yl : Loc⸩ => {i}]
   {
     [∗ in ⟪0,pay_index⟫ ∪ ⟪1,lang_index⟫ | xl ~~> xv ∗ yl ~~> yv]
   }
-  [0| p in pay_index => prog_c1(⸨xl : Loc⸩, ⸨yl : Loc⸩, ⟨p.val.2.1⟩, ⟨p.val.2.2⟩) ]
-  [1| l in lang_index => l.val.fst(⸨xl: Loc⸩, ⸨yl : Loc⸩)]
+  [0| p in pay_index => prog_c1(⸨xl : Loc⸩, ⸨yl : Loc⸩, ⟨Int.ofNat p.val.2.1⟩, ⟨p.val.2.2⟩) ]
+  [1| l in lang_index => ⌜ tfunc l.val.fst ⌝(⸨xl: Loc⸩, ⸨yl : Loc⸩)]
   { v,
     fun h => ∀ ll ∈ lang_index, ∃ pp ∈ pay_index , h ⟨1, ll⟩ = h ⟨0, pp⟩
   }
   := by
-  unfold LGTM.triple
-  rw [← bighstar_hhstar_disj_dir (s₁ := ⟪0, pay_index⟫) (s₂ := ⟪1, lang_index⟫ ) ]
-  rotate_left
-  apply disjoint_label_set.mpr; simp; rfl
-  rw [← bighstar_hhstar_disj_dir (s₁ := ⟪1, lang_index1⟫ ) (s₂ := ⟪1, lang_index2⟫ ) (s := ⟪1, lang_index⟫)]
-  rotate_left
-  apply disjoint_label_set.mpr; right; apply lang_disjoint;
-  rw [lang_union]; unfold labSet; aesop
-  -- Step 1 : GrmDisj rule
-  apply weird_grmdisj_lemma_standard (s1 := lang_index1) (s2 := lang_index2) (s' := pay_index)
-  rfl; rfl; apply disjoint_label_set.mpr; simp; apply Set.disjoint_iff_inter_eq_empty.mp lang_disjoint; apply eq_comm.mpr lang_union
-  simp; simp; simp
-  · rw [← bighstar_hhstar_disj_dir (s₁ := ⟪0, pay_index2⟫) (s₂ := ⟪0, pay_index1⟫ )]
-    rotate_left
-    apply disjoint_label_set.mpr; simp; apply disjoint_comm.mpr pay_disjoint; rw [labSet_union]; rw [Set.union_comm]; apply pay_union
-    rw [hhstar_assoc]
+  intro tfunc
+  yin 1 :
+    try (first
+      | (apply ywp_lemma_funs;
+         { move=> ?; rfl }
+         { move=> ?; rfl }
+         { move=> ?; rfl }
+         { move=> ?; simp [Unary.get_vars, Unary.type_match] } ))
+  yin 0 :
+    try (first
+      | (apply ywp_lemma_funs;
+         { move=> ?; rfl }
+         { move=> ?; rfl }
+         { move=> ?; rfl }
+         { move=> ?; simp [Unary.get_vars, Unary.type_match] } ))
+  dsimp [Unary.func_call_ctx_prepare]
+  try simp [isubstE, Unary.reduce_call_isubst]
+  clear tfunc
 
-    -- Step 2: Weaken rule
-    apply weird_weaken_lemma' (s' := pay_index1)=>//
-    { have tmp := pay_union
-      simp_all only [Set.subset_union_left] }
-    { simp; apply disjoint_label_set.mpr; simp }
-    {
-      -- Prove the termination of the useless part
-      dsimp
-      have tmp : pay_index2 = pay_index \ pay_index1 := by
-        rw [pay_union]; simp
-        exact Eq.symm (Disjoint.sdiff_eq_right pay_disjoint)
-      rw [←tmp]
-      dsimp [LGTM.wp, LGTM.SHTs.htrm]
-      rw [hwp_ht_eq (ht₂ := (fun (p : (trm × payload × payload)ˡ) => prog_c1.trm_call [xl, yl, [lang| ⟨p.val.2.1⟩], [lang| ⟨p.val.2.2⟩]] ))] --remove union set
-      on_goal 2=> simp only [Set.EqOn, fun_insert, Set.union_empty] ; intro a b ; simp only [b, reduceIte]
-      unfold prog_c1
-      have tmp := htriple_prod (α := (trm × payload × payload)ˡ) (s := ⟪0, pay_index2⟫)
-        (ht := open Classical in (fun a => prog_c1.trm_call [xl, yl, [lang| ⟨a.val.2.1⟩], [lang| ⟨a.val.2.2⟩]]))
-        (H := fun _ => xl ~~> xv ∗ yl ~~> yv)
-        (Q := fun i v => fun h => ∀ a ∉ ⟪0, pay_index2⟫, h = ∅)
-      specialize tmp (by
-        clear tmp
-        intro a ha
-        unfold prog_c1
-        xwp ; xseq_xlet_if_needed
-        by_cases hav : a.val.2.1 ≥ 0
-        {
-          stop -- faster for debugging
-          xfor (fun a => xl ~~> ((xv + a) : ℤ))
-          · intro i hi hia
-            xstep; xwp; xlet; xstep; xapp; xsimp
-          · intro _; dsimp
-            xwp; xseq
-            xfor (fun a => yl ~~> ((yv + a) : ℤ))
-            {
-              intro i hi hia; xwp; xlet;
-              xapp; xwp; xlet; xapp; xapp; xsimp
-            }
-            intro _; dsimp
-            xwp; xlet;
-            xapp; xwp; xlet; xapp
-            xwp; xlet;
-            apply triple_conseq_frame ; apply triple_gt ; xsimp;
-            intro k; dsimp;
-            xsimp_start -- something wrong with xsimp here
-            xsimp_step
-            -- apply xsimp_r_hpure;
-            -- xsimp_step
-            -- xsimp_step
-            -- xsimp_step
-            -- xsimp_step
-            -- try rev_pure
-            -- try hide_mvars
-            -- try hsimp
-            -- rotate_left
-            sorry
-        }
-        {
-          stop -- faster for debugging
-          apply xfor_empty_lemma
-          { simp_all [not_le, gt_iff_lt] }
-          intro _; dsimp
-          xwp; xseq
-          apply xfor_empty_lemma
-          { simp_all [not_le, gt_iff_lt] }
-          intro _; dsimp
-          xwp; xlet; xapp; xwp; xlet; xapp; xwp; xlet
-          apply triple_conseq_frame ; apply triple_gt ; xsimp;
-          intro k; dsimp;
-          xsimp -- something wrong with xsimp here
-        }
-      )
-      apply hhimpl_trans ; apply tmp
-      clear tmp
-      rw [Set.union_empty]
-      unfold prog_c1;
-      apply hwp_conseq
-      unfold bighstar bighstarDef;
-      intro hv hh pre a ha;
-      specialize pre a
-      simp [ha] at pre
-      assumption
-    }
-    {
-      -- Step 3: InfDisj rule
-      dsimp
-      stop
-      -- need to use ymerge to merge all positive p.val.2.2
-      apply ymerge_lemma
-        («μ» := fun x => (x.1, (x.2.1, 10)))
-        (t := pay_index1) (l := 0)
-        (H' := [∗i in ⟪1, lang_index1⟫| xl ~~> xv ∗ yl ~~> yv])
+  -- for simplicity, use the axiom of choice to build the oracle
+  have tmp := fun_union_exists (fun n => Set.singleton
+    ([lang| fun ⸨xl: Loc⸩ ⸨yl : Loc⸩ => { (lang_sn1 n) }])) Set.univ
+  specialize tmp ?_
+  { simp ; intro i j hneq ; simp [Set.singleton, trm_funs, lang_sn1]
+    intro heq ; apply Example3.cfgexp_grammar_injective at heq
+    · contradiction
+    · unfold Example3.trm1 ; simp
+    · unfold Example3.trm2 ; simp
+  }
+  rcases tmp with ⟨aux, haux⟩ ; simp [Set.singleton] at haux
 
-      ymerge 0 with (μ := fun x => (x.1, (x.2.1, 10)))
-
-      stop
-      apply weird_infdisj_lemma (s1 := pay_index1) (s2 := lang_index1) (Hx := xl ~~> xv ∗ yl ~~> yv)
-        (f := fun i => (default_trm, Int.ofNat i))
-        (g := fun i => ([lang| fun ⸨xl: Loc⸩ ⸨yl : Loc⸩ => {trm_seq (cfgexp_grammar i trm1 trm2) (trm3)}],default_payload))
-        (Idx := @Set.univ ℕ)
-      rfl; rfl; unfold pay_index1; simp;
-      sorry
+  apply LGTM.triple_conseq-- ; apply hhimpl_refl ; rotate_left
+  rotate_left ; rotate_left
+  apply weird_gram_seq_full_prod
+    (α := (trm × Example3.payload × payload)ˡ)
+    (β := (trm × Example3.payload)ˡ)
+    (γ := (trm × payload)ˡ)
+    (sht_prog1 := LGTM.SHT.mk ⟪0, Example3.pay_index⟫
+      fun p ↦ Example3.prog_c1.trm_call [xl, yl, [lang| ⟨Int.ofNat p.val.2⟩]])
+    (sht_lang1 := LGTM.SHT.mk ⟪1, Example3.lang_index⟫
+      fun l ↦ l.val.1.trm_call [xl, yl])
+    (sht_prog2 := LGTM.SHT.mk ⟪0, Example0.pay_index⟫
+      fun p ↦ Example0.prog_c1.trm_call [xl, yl, [lang| ⟨p.val.2⟩]])
+    (sht_lang2 := LGTM.SHT.mk ⟪1, Example0.lang_index⟫
+      fun l ↦ l.val.1.trm_call [xl, yl])
+    (proj1 := fun a => ⟨a.lab, (trm_call_fun <| trm_seq_fst a.val.1, a.val.2.1)⟩)
+    (proj2 := fun a => ⟨a.lab, (trm_call_fun <| trm_seq_snd a.val.1, a.val.2.2)⟩)
+    (part1_oracle := fun a => ⟨0, (default_trm, aux a.val.1 |>.getD 0)⟩)
+    (H1 := fun _ => xl ~~> xv ∗ yl ~~> yv)
+    (Q1 := fun n =>
+      hforall fun j =>
+      hforall fun (_ :
+      n ∈ (({⟨0, (default_trm, j)⟩} ∪
+      {⟨1, ([lang| fun ⸨xl: Loc⸩ ⸨yl : Loc⸩=> {Example3.cfgexp_grammar j Example3.trm1 Example3.trm2}], Example3.default_payload)⟩}) : Set (trm × Example3.payload)ˡ)) =>
+      (xl ~~> (xv + Int.ofNat j) ∗ yl ~~> (yv + Int.ofNat j)))
+  { simp [lang_index, lang_squeeze_list']
+    exists (((lang_part1 0).trm_seq (lang_part2 false)), Example3.default_payload, default_payload)
+    simp }
+  { simp [pay_index] ; exists (default_trm, Nat.zero, 0) ; simp }
+  { clear aux haux
+    ext a ; dsimp only ; rcases a with ⟨⟨al, ⟨atrm, ap⟩⟩, ⟨bl, ⟨btrm, bp⟩⟩⟩
+    simp [lang_index, lang_squeeze_list',
+      Example3.lang_index, Example3.lang_fun_list, Example3.lang_squeeze_list,
+      Example0.lang_index, Example0.lang_index'_unfold,
+      lang_part1, lang_part2]
+    simp [← lang_sn1.eq_1, exists_labType, Bool.exists_bool, orexp_grammar]
+    constructor
+    · intro h ; aesop
+    · intro h ; exists 1 ; aesop
+  }
+  { clear aux haux
+    ext a ; dsimp only ; rcases a with ⟨⟨al, ⟨atrm, ap⟩⟩, ⟨bl, ⟨btrm, bp⟩⟩⟩
+    simp [pay_index,
+      Example3.pay_index,
+      Example0.pay_index, Example0.pay_index',
+      default_trm]
+    simp [exists_labType]
+    aesop
+  }
+  { rw [disjoint_label_set] ; left ; decide }
+  { rw [disjoint_label_set] ; left ; decide }
+  { rw [disjoint_label_set] ; left ; decide }
+  { simp ; ext a ; rcases a with ⟨al, ⟨atrm, ap⟩⟩
+    simp [Example3.pay_index, Example3.lang_index, Example3.lang_fun_list, Example3.lang_squeeze_list,
+      exists_labType, ← lang_sn1.eq_1]
+    constructor
+    { rintro ⟨_, _⟩ ; subst al atrm
+      exists 1, trm_funs [trm_varl "xl", trm_varl "yl"] (lang_sn1 ap)
+      simp ; rw [(haux _ ap).mp rfl] ; rfl
     }
-  · rw [← bighstar_hhstar_disj_dir (s₁ := ⟪0, pay_index1⟫) (s₂ := ⟪0, pay_index2⟫ )]
-    rotate_left
-    apply disjoint_label_set.mpr; simp; apply pay_disjoint; rw [labSet_union]; apply pay_union
-    rw [hhstar_assoc]
-    apply weird_weaken_lemma' (s' := pay_index2)=>//
-    { have tmp := pay_union
-      simp_all only [Set.subset_union_right] }
-    { simp; apply disjoint_label_set.mpr; simp }
-    {
-      -- same issue as the Step 2 above
-      sorry
+    { simp ; intros ; subst_eqs ; simp }
+  }
+  { dsimp only
+    rintro hh hpre ⟨ll, ⟨ltrm, lp⟩⟩ lin
+    -- on the lang side first
+    whnf at hpre ; unfold hforall at hpre ; dsimp at hpre
+    have hpre' := hpre ⟨ll, ⟨ltrm, lp⟩⟩ ; rw [if_pos] at hpre'
+    on_goal 2=> simp only [Set.mem_union] ; right ; assumption
+    simp [Example3.lang_index, Example3.lang_fun_list, Example3.lang_squeeze_list] at lin
+    rcases lin with ⟨_, ⟨n, lin⟩, _⟩ ; subst ll lp ; dsimp
+    specialize hpre' n (by subst ltrm ; simp)
+    -- on the payload side
+    specialize hpre ⟨0, ⟨default_trm, n⟩⟩ ; rw [if_pos] at hpre
+    on_goal 2=> simp [Example3.pay_index]
+    specialize hpre n (by simp)
+    constructor
+    on_goal 1=> simp [Example3.pay_index]
+    -- trick
+    have tmp := HPropExact.isExact _ _ hpre' hpre
+    rw [(haux ltrm n).mp (by subst ltrm ; rfl)] ; exact tmp
+  }
+  { dsimp
+    rintro ⟨il, ⟨itrm, ip⟩⟩ hin
+    simp [Example3.pay_index, Example3.lang_index, Example3.lang_fun_list, Example3.lang_squeeze_list] at hin
+    constructor
+    intro he1 he2 h1 h2 ; simp [hforall] at h1 h2
+    rcases hin with (hin | hin)
+    · specialize h1 ip (by left ; simp [hin])
+      specialize h2 ip (by left ; simp [hin])
+      have tmp := HPropExact.isExact _ _ h1 h2 ; exact tmp
+    · rcases hin with ⟨_, ⟨n, hin⟩, _⟩ ; subst_eqs ; simp at h1 h2
+      specialize h1 n rfl ; specialize h2 n rfl
+      have tmp := HPropExact.isExact _ _ h1 h2 ; exact tmp
+  }
+  { dsimp only
+    rintro ⟨al, ⟨atrm, ap1, ap2⟩⟩ ; dsimp
+    intro hin ; simp [lang_index, lang_squeeze_list'] at hin
+    rcases hin with ⟨_, ⟨p1, p2, _⟩, _, _⟩ ; subst_eqs
+    dsimp only [trm_call_fun, trm_seq_fst, trm_seq_snd, lang_part1, lang_part2, trm_funs, lang_sn1]
+    -- bug ????
+    -- simp [isubstE]
+    dsimp only [isubst, isubst.go] ; congr! 1
+    { congr! 3 ; rw [Example3.cfgexp_grammar_isubst] ; rfl }
+    { cases p2 <;> rfl }
+  }
+  { simp }
+  { apply Example3.example3_spec_ }
+  { rintro ⟨jl, ⟨jtrm, jp⟩⟩ jin
+    simp [Example3.pay_index, Example3.lang_index, Example3.lang_fun_list, Example3.lang_squeeze_list] at jin
+    rcases jin with ⟨_, ⟨n, jin⟩, _⟩ ; subst jl jp ; symm at jin
+    dsimp only
+    -- involving the oracle here
+    apply LGTM.triple_conseq
+    on_goal 3=> apply Example0.example1_spec (xv + Int.ofNat (aux jtrm |>.getD 0)) (yv + Int.ofNat (aux jtrm |>.getD 0))
+    { apply bighstar_himpl
+      intro a ain hh hpre ; simp [hforall] at hpre ; specialize hpre n jin
+      rw [(haux jtrm n).mp jin] ; exact hpre
     }
-    {
-      -- Step 3: InfDisj rule
-      sorry
+    { intro hv hh hpre ; simp
+      rintro ⟨ll, ⟨ltrm, lp⟩⟩ lin ; simp at lin ; subst ll
+      simp [Example0.lang_index, Example0.lang_index'_unfold, Example0.pay_index, exists_labType] at hpre ⊢
+      intro h ; apply hpre at h
+      clear *- h ; aesop
     }
+  }
+  { simp }
+  { simp [forall_labType, exists_labType, lang_index, lang_squeeze_list', pay_index]
+    intro hv hh hpre a b c d ; specialize hpre _ a b c rfl d ; exact hpre
+  }
 
 /- Previously, constraints for payloads in the heap are in the post-condition
     -- ∧ arr⟨{⟨0,p⟩}⟩(pa , i in pa_len => p.2.1[i]!) h
