WeirdLogic/Example3_1.lean
@@ -1,0 +1,620 @@
+import Mathlib.Computability.ContextFreeGrammar
+
+import Lgtm.Hyper.ProofMode
+import Lgtm.Hyper.ArraysFun
+import Lgtm.Unary.Lang
+import Lgtm.Experiments.HyperCommon
+
+import WeirdLogic.Gram
+import WeirdLogic.WLogic
+import WeirdLogic.WTriple
+import WeirdLogic.WUtil
+import WeirdLogic.Hete
+import WeirdLogic.WUnary
+
+open Unary prim val trm
+open ContextFreeGrammar
+
+namespace WeirdLogic.Example3
+
+/- L -> (S1)
+  S1 -> trm1; S1; trm2
+        | ε
+
+  L = {trm1ⁿ;trm2ⁿ : n ≥ 0}
+  context free + infdisj rule -/
+def trm1 : trm := [lang| let xx := !xl in let temp0 := xx + 1 in xl := temp0]
+def trm2 : trm := [lang| let yy := !yl in let temp1 := yy + 1 in yl := temp1]
+def r1 : ContextFreeRule trm String :=
+  {
+    input := "L",
+    output := [Symbol.nonterminal "S1"]
+  }
+
+def r2 : ContextFreeRule trm String :=
+  {
+    input := "S1",
+    output := [Symbol.terminal trm1, Symbol.nonterminal "S1", Symbol.terminal trm2],
+  }
+
+def r3 : ContextFreeRule trm String :=
+  {
+    input := "S1",
+    output := [],
+  }
+
+
+def cfg1 : ContextFreeGrammar trm :=
+  {
+    NT := String,
+    initial := "S1",
+    rules := Finset.mk {r1, r2, r3} (by unfold r1 r2 r3 trm1 trm2; simp)
+  }
+
+def l1 : Language trm := cfg1.language
+
+def cfg_expand : Set ( List (Symbol T N)) :=
+  {
+    c | cfg1.Generates c
+  }
+
+lang_def prog_c1 :=
+  fun ⸨xl: Loc⸩ ⸨yl: Loc⸩ ⸨pa:Val⸩ =>
+    for k in [0:pa] {
+      let xx := !xl in
+      let temp0 := xx + 1 in
+      xl := temp0
+    };
+    for j in [0:pa] {
+      let yy := !yl in
+      let temp1 := yy + 1 in
+      yl := temp1
+    }
+
+abbrev Lang := List trm
+
+def lang_list_index : Set (List trm) :=
+  {l | (trm_to_symbol_list l) ∈ cfg_expand }
+
+def regexp_grammar : ℕ → trm → trm
+  | 0, _ => trm_val val_unit
+  | 1, t => t
+  | (n+1), t => trm_seq t (regexp_grammar n t)
+
+def cfgexp_grammar : ℕ → trm → trm → trm
+  | 0, _, _ => trm_val val_unit
+  | n, t1, t2 => trm_seq (regexp_grammar n t1) (regexp_grammar n t2)
+  -- | 1, t1, t2 => trm_seq t1 t2
+  -- | (n+1), t1, t2 => trm_seq t1 (trm_seq (cfgexp_grammar n t1 t2) t2)
+
+def lang_squeeze_list: Set trm :=
+  {cfgexp_grammar i trm1 trm2 | i : ℕ }
+
+def lang_fun_list : Set trm :=
+  {[lang| fun ⸨xl: Loc⸩ ⸨yl : Loc⸩ => {tt}] | tt ∈ lang_squeeze_list }
+
+-- TODO for now, to keep things mostly feasible, we restrict the payload to `ℕ`
+
+def payload := Nat
+def default_payload := 0
+
+def pay_index : Set (trm × payload) :=
+  {
+    (default_trm,p) | p ∈ @Set.univ payload
+  }
+
+def lang_index : Set (trm × payload ):=
+  { (l,default_payload) | l ∈ lang_fun_list }
+
+variable (pa_len : ℕ) (pb_len : ℕ) (xptr : loc)
+variable (paptr : trm × payload -> loc) (pbptr : trm × payload -> loc)
+
+lemma regexp_grammar_isubst (n : ℕ) (t : trm) :
+  isubst Ev El (regexp_grammar n t) = regexp_grammar n (isubst Ev El t) := by
+  fun_induction regexp_grammar n t
+  all_goals simp [regexp_grammar, isubst]
+  assumption
+
+lemma cfgexp_grammar_isubst (n : ℕ) (t1 t2 : trm) :
+  isubst Ev El (cfgexp_grammar n t1 t2) = cfgexp_grammar n (isubst Ev El t1) (isubst Ev El t2):= by
+  unfold cfgexp_grammar
+  cases n
+  case zero => simp [isubst]
+  case succ n =>
+    simp [isubst]
+    constructor <;> apply regexp_grammar_isubst
+  -- proofs if use old format
+  -- fun_induction cfgexp_grammar n t1 t2
+  -- all_goals simp [cfgexp_grammar, isubst]
+  -- assumption
+
+
+lemma equiv_1 (a : Int)
+  (h : ∀ (v : val), subst i v t = t)
+  (hQ : (∀ v1 v2, Q v1 = Q v2))
+  :
+  eval s (regexp_grammar n t) Q ↔ eval s (trm_for i a ((a + n : Int)) t) Q := by
+  fun_induction regexp_grammar n t generalizing s a
+  next t =>
+    simp [regexp_grammar] ; rw [empty_for_loop, eval_for_val]
+  next t =>
+    simp [regexp_grammar]
+    constructor
+    · intro hh ; constructor ; simp ; rw [h]
+      constructor ; assumption
+      intros ; rw [empty_for_loop, hQ] ; assumption
+    · intro hh ; cases hh ; rename_i hh
+      simp at hh ; rw [h] at hh
+      cases hh ; rename_i Q1 hmid h2
+      simp only [empty_for_loop] at h2
+      apply eval_conseq' ; assumption
+      intros ; rw [hQ _ val_unit] ; solve_by_elim
+  next n t not0 ih =>
+    have tmp : a + 1 + ↑n = a + (↑n + 1) := by ac_rfl
+    simp [regexp_grammar]
+    constructor
+    · intro hh ; constructor ; simp ; rw [h]
+      cases hh ; rename_i Q1 hmid h2
+      constructor ; assumption
+      intro v1 s2 h2_ ; specialize h2 _ _ h2_
+      specialize @ih s2 (a + 1) h ; rw [tmp] at ih
+      rw [← ih] ; assumption
+    · intro hh ; cases hh ; rename_i hh
+      simp at hh ; rw [h] at hh
+      cases hh ; rename_i Q1 hmid h2
+      constructor ; assumption
+      intro v1 s2 h2_ ; specialize h2 _ _ h2_
+      specialize @ih s2 (a + 1) h ; rw [tmp] at ih
+      rw [ih] ; assumption
+
+lemma simple_loop_pre (xl : loc) (xv : ℤ) (n : Nat) :
+  let nn : val := val_int n
+  triple
+    [lang|
+      for k in [0 : nn] {
+        let xx := !xl in
+        let temp0 := xx + 1 in
+        xl := temp0
+      }]
+    (xl ~~> xv) (fun _ => xl ~~> ((xv + n) : ℤ)) := by
+  xfor (fun a => xl ~~> ((xv + a) : ℤ))
+  intro i h1 h2 ; xwp ; xlet
+  on_goal 2=> xsimp ; xsimp
+  xapp ; xwp ; xlet ; xstep ; xapp ; xsimp
+
+lemma simple_loop_pre2 (xl : loc) (xv : ℤ) (yv : ℤ) (n : Nat) :
+  let nn : val := val_int n
+  triple
+    [lang|
+      for k in [0 : nn] {
+        let xx := !xl in
+        let temp0 := xx + 1 in
+        xl := temp0
+      }]
+    (xl ~~> xv ∗ yl ~~>yv)
+    (fun _ => xl ~~> ((xv + n) : ℤ) ∗ yl ~~> yv) := by
+  apply triple_frame
+  apply simple_loop_pre
+
+lemma simple_loop_pre3 (xl : loc) (xv : ℤ) (yv : ℤ) (n : Nat) :
+  let nn : val := val_int n
+  triple
+    [lang|
+      for k in [0 : nn] {
+        let yy := !yl in
+        let temp1 := yy + 1 in
+        yl := temp1
+      }]
+    (xl ~~> ((xv + n) : ℤ)∗ yl ~~>yv)
+    (fun _ => yl ~~> ((yv + n) : ℤ)∗ xl ~~> ((xv + n) : ℤ)) := by
+  rw [hstar_comm]
+  apply triple_frame
+  xfor (fun a => yl ~~> ((yv + a) : ℤ))
+  intro i h1 h2 ; xwp ; xlet
+  on_goal 2=> xsimp ; xsimp
+  xapp ; xwp ; xlet ; xstep ; xapp ; xsimp
+
+lemma example3_single_iter (xv : ℤ) (yv : ℤ):
+  ∀ n : ℕ,
+  sn = [lang| fun ⸨xl: Loc⸩ ⸨yl : Loc⸩=> {cfgexp_grammar n trm1 trm2}] →
+  [∗ in {⟨0, (default_trm, n)⟩} ∪ {⟨1, (sn, default_payload)⟩}| xl ~~> xv ∗ yl ~~> yv] ==>
+  LGTM.wp
+    [{ s := ⟪0, {(default_trm, n)}⟫, ht := fun p ↦ prog_c1.trm_call [xl, yl, [lang| ⟨Int.ofNat p.val.2⟩]] },
+     { s := ⟪1, {(sn, default_payload)}⟫, ht := fun l ↦ l.val.1.trm_call [xl, yl] }]
+    fun _ =>
+      -- h => ∀ l ∈ ({(sn, default_payload)} : Set (trm × payload)), ∃ p ∈ ({(default_trm, n)} : Set (trm × payload)), h ⟨1, l⟩ = h ⟨0, p⟩
+      [∗ in {⟨0, (default_trm, n)⟩} ∪ {⟨1, (sn, default_payload)⟩}| xl ~~> (xv + n) ∗ yl ~~> (yv + n)]
+  := by
+  intro n hsn
+  unfold LGTM.wp labSet
+  open Classical in simp +unfoldPartialApp [fun_insert]
+  have tmp := htriple_prod (α := (trm × payload)ˡ) (s := {⟨1, (sn, default_payload)⟩, ⟨0, (default_trm, ↑n)⟩})
+    (ht := open Classical in (fun a =>
+      if a = ⟨0, (default_trm, ↑n)⟩ then prog_c1.trm_call [xl, yl, [lang| ⟨Int.ofNat a.val.2⟩]]
+      else if a = ⟨1, (sn, default_payload)⟩ then a.val.1.trm_call [xl, yl] else [lang| ()]))
+    (H := fun _ => xl ~~> xv ∗ yl ~~> yv)
+    (Q := fun _ _ => xl ~~> ((xv + n) : ℤ) ∗ yl ~~> ((yv + n) : ℤ) )
+  specialize tmp (by
+    clear tmp
+    simp
+    constructor
+    · rw [hsn] ;
+      (apply xwp_lemma_funs'; rfl; rfl; { simp [get_vars, type_match];}; { rfl })
+      rw [cfgexp_grammar_isubst, trm1, trm2] ; simp [isubst, isubst.go]
+      intro h hh ;
+      unfold cfgexp_grammar
+      cases n
+      case zero =>
+        simp;
+        revert h hh
+        apply empty_pre (H := xl ~~> xv ∗ yl ~~> yv)
+      case succ n =>
+        simp
+        xwp; xseq_xlet_if_needed;
+        intro h hh ; apply (equiv_1 (i := "k") 0 _ _).mpr
+        on_goal 2=> intro v ; rfl
+        on_goal 2=> intros ; rfl
+        on_goal 2=> exact hh
+        simp ;
+        -- revert h hh
+        have tpre := simple_loop_pre2 (xv := xv) (yl := yl) (xl := xl) (yv := yv) (n := n+1) h hh
+        apply eval_conseq=>//
+        intro v; simp
+        intro h hh ; apply (equiv_1 (i := "k") 0 _ _).mpr
+        on_goal 2=> intro v ; rfl
+        on_goal 2=> intros ; rfl
+        clear tpre
+        -- revert h hh
+        have tpre := simple_loop_pre3 (xv := xv) (yl := yl) (xl := xl) (yv := yv) (n := n+1) h hh
+        apply eval_conseq (Q1 := fun x ↦ yl ~~> val_int (yv + ↑(n + 1)) ∗ xl ~~> val_int (xv + ↑(n + 1)))=>//
+        intro v; simp
+        rw [hstar_comm]; simp
+    · xwp; xseq_xlet_if_needed;
+      xfor (fun a => xl ~~> ((xv + a) : ℤ))
+      -- exact Nat.cast_nonneg n;
+      intro i h1 h2 ; xwp ; xlet;
+      · xapp ; xwp ; xlet ; xstep ; xapp ; xsimp
+      · intro h; simp
+        xfor (fun a => yl ~~> ((yv + a) : ℤ))
+        -- · exact Nat.cast_nonneg n;
+        intro i h1 h2 ; xwp ; xlet;
+        · xapp ; xwp ; xlet ; xstep ; xapp ; xsimp
+        · xsimp ; xsimp;
+  )
+  assumption
+  -- apply hhimpl_trans ; apply tmp
+  -- clear tmp
+  -- apply hwp_conseq
+  -- ysimp
+  -- unfold bighstar bighstarDef ; open Classical in simp
+  -- intro h hh
+  -- have h1 := hh ⟨1, (trm_funs [trm_varl "xl", trm_varl "yl"] (cfgexp_grammar n trm1 trm2), 0)⟩ ; simp at h1
+  -- have h2 := hh ⟨0, (default_trm, ↑n)⟩ ; simp at h2
+  -- unfold hsingle at h1 h2;
+
+  -- unfold HStar.hStar instHStarHProp at h1 h2; simp at h1 h2
+  -- unfold hstar at h1 h2 ;
+  -- rcases h1 with ⟨h11,h12,hh1,hh2,hh3,hh4⟩
+  -- rcases h2 with ⟨h21,h22,hh21,hh22,hh23,hh24⟩
+  -- rw [hh24,hh4,hh1,hh2,hh21,hh22]
+
+
+def regexp_grammar_injective ( i j : ℕ) ( t : trm):
+  t ≠ [lang| ()] ->
+  regexp_grammar i t =  regexp_grammar j t ->
+  i = j := by
+  intro ht h
+  unfold regexp_grammar at h
+  induction i generalizing j with
+  | zero =>
+    induction j with
+    | zero => rfl
+    | succ jn hjn =>
+        cases jn
+        case zero => simp_all
+        case succ jj => simp_all
+  | succ ik hik=>
+    induction j with
+    | zero =>
+        cases ik
+        case zero => simp_all
+        case succ jj => simp_all
+    | succ jn hjn =>
+        simp
+        cases ik
+        case zero =>
+          cases jn
+          case zero => simp_all
+          case succ jnn =>
+            simp only [Nat.zero_add, Nat.add_zero] at h
+            have tnq := trm_seq_neq t (regexp_grammar (jnn + 1) t)
+            contradiction
+        case succ ikk =>
+          cases jn
+          case zero =>
+            simp only [Nat.zero_add, Nat.add_zero] at h
+            have tnq := trm_seq_neq t (regexp_grammar (ikk + 1) t)
+            simp_all
+          case succ jnn =>
+            simp_all
+            unfold regexp_grammar at h
+            specialize hik (jnn+1) h
+            simp_all
+
+def cfgexp_grammar_injective ( i j : ℕ) ( t1 t2 : trm):
+  t1 ≠ [lang| ()] -> t2 ≠ [lang| ()] ->
+  cfgexp_grammar i t1 t2 =  cfgexp_grammar j t1 t2 ->
+  i = j := by
+  intro ht1 ht2 h
+  cases i
+  case zero =>
+    cases j
+    case zero => simp
+    case succ j1=>
+      unfold cfgexp_grammar at h
+      simp_all
+  case succ i1 =>
+    cases j
+    case zero => unfold cfgexp_grammar at h; simp_all
+    case succ j1 =>
+      unfold cfgexp_grammar at h; simp [*] at h
+      rcases h with ⟨h1,h2⟩
+      apply regexp_grammar_injective at h1
+      repeat assumption
+
+set_option maxRecDepth 2000 in
+set_option maxHeartbeats 6400000 in
+lemma example3_spec_ (xv yv : ℤ) :
+  {
+    [∗ in ⟪0,pay_index⟫ ∪ ⟪1,lang_index⟫ | xl ~~> xv ∗ yl ~~> yv]
+  }
+  [0| p in pay_index => prog_c1(⸨xl : Loc⸩, ⸨yl : Loc⸩, ⟨Int.ofNat p.val.2⟩) ]
+  [1| l in lang_index => l.val.fst(⸨xl: Loc⸩, ⸨yl : Loc⸩)]
+  { v,
+    -- fun h => ∀ ll ∈ lang_index, ∃ pp ∈ pay_index , h ⟨1, ll⟩ = h ⟨0, pp⟩
+    -- [∗ in
+    --   ⋃ (n : payload), ({⟨0, (default_trm, n)⟩} ∪
+    --   {⟨1, ([lang| fun ⸨xl: Loc⸩ ⸨yl : Loc⸩=> {cfgexp_grammar n trm1 trm2}], default_payload)⟩}) |
+    --   xl ~~> (xv + Int.ofNat n) ∗ yl ~~> (yv + Int.ofNat n)]
+    [∗ n in ⟪0,pay_index⟫ ∪ ⟪1,lang_index⟫
+      -- ⋃ (i : payload), ({⟨0, (default_trm, i)⟩} ∪
+      -- {⟨1, ([lang| fun ⸨xl: Loc⸩ ⸨yl : Loc⸩=> {cfgexp_grammar i trm1 trm2}], default_payload)⟩})
+      |
+      hforall fun j =>
+      hforall fun (_ :
+      n ∈ (({⟨0, (default_trm, j)⟩} ∪
+      {⟨1, ([lang| fun ⸨xl: Loc⸩ ⸨yl : Loc⸩=> {cfgexp_grammar j trm1 trm2}], default_payload)⟩}) : Set (trm × payload)ˡ)) =>
+      (xl ~~> (xv + Int.ofNat j) ∗ yl ~~> (yv + Int.ofNat j))
+    ]
+  }
+  := by
+  unfold LGTM.triple
+  /-
+  rw [← bighstar_hhstar_disj_dir (s₁ := {⟨0,(default_trm,p)⟩ | p <0 }) (s₂ := {⟨0,(default_trm,p)⟩ | p ≥ 0} ∪ ⟪1, lang_index⟫ )]
+  rotate_left
+  { apply Set.disjoint_union_right.mpr
+    simp;
+    constructor
+    · srw Set.disjoint_iff_inter_eq_empty Set.eq_empty_iff_forall_notMem=>x//==
+      move=> x1 h1 [x2] h2 Z; cases Z
+      exact lt_irrefl x1 (lt_of_lt_of_le h1 h2)
+    · unfold labSet
+      srw Set.disjoint_iff_inter_eq_empty Set.eq_empty_iff_forall_notMem=>x//==
+      move=>y1 H1 [y2] H2 Z; cases Z
+      simp
+  }
+  { rw [←Set.union_assoc]
+    apply Set.union_eq_union_iff_right.mpr
+    have eq : {x | ∃ p < 0, ⟨0, (default_trm, p)⟩ = x} ∪ {x | ∃ p ≥ 0, ⟨0, (default_trm, p)⟩ = x} = ⟪0, pay_index⟫ := by
+      unfold labSet pay_index
+      ext x
+      constructor
+      · intro hx
+        rcases hx with ⟨p, hp, rfl⟩ | ⟨p, hp, rfl⟩
+        · simp;
+        · simp
+      · intro hx
+        rcases hx with ⟨p, hp, rfl⟩
+        simp_all only [Set.mem_univ, true_and, Set.mem_setOf_eq, ge_iff_le, Set.mem_union, Labeled.mk.injEq]
+        obtain ⟨fst, snd⟩ := p
+        obtain ⟨w, h⟩ := hp
+        simp_all only [Prod.mk.injEq, true_and, exists_eq_right]
+        obtain ⟨left, right⟩ := h
+        subst right left
+        exact lt_or_ge w 0
+    rw [eq]
+    constructor <;> apply Set.subset_union_left
+  }
+  -/
+  set Hx := xl ~~> xv ∗ yl ~~> yv with hhx
+  /-
+  /- Step 1: remove negative cases-/
+  apply weird_weaken_lemma' (s' := {(default_trm,p) | p ≥ 0 })=>//
+  unfold pay_index; simp; simp; apply disjoint_label_set.mpr; simp
+  {
+    dsimp [LGTM.wp, LGTM.SHTs.htrm]
+    rw [hwp_ht_eq (ht₂ := (fun (p : (trm × payload)ˡ) => prog_c1.trm_call [xl, yl, [lang| ⟨p.val.2⟩]]))] --remove union set
+    on_goal 2=> simp only [Set.EqOn, fun_insert, Set.union_empty] ; intro a b ; simp only [b, reduceIte]
+    have tmp := htriple_prod (α := (trm × payload)ˡ) (s := ⟪0, pay_index \ {x | ∃ p ≥ 0, (default_trm, p) = x}⟫ ∪ ∅)
+      (ht := open Classical in (fun a => prog_c1.trm_call [xl, yl, [lang| ⟨a.val.2⟩]]))
+      (H := fun _ => Hx)
+      (Q := fun i v => fun h => i ∉ ⟪0, {x | ∃ p <0, (default_trm, p) = x}⟫ -> h = ∅)
+    specialize tmp (by
+      clear tmp
+      intro a ha
+      unfold Hx prog_c1
+      xwp; xseq_xlet_if_needed;
+      apply xfor_empty_lemma
+      {
+        simp [pay_index] at ha
+        rcases ha with ⟨ ha1,⟨p,ha2⟩,ha3⟩
+        specialize ha3 p
+        simp_all
+        rw [←ha2]
+        simp
+        assumption
+      }
+      intro x
+      dsimp
+      apply xfor_empty_lemma
+      {
+        simp [pay_index] at ha
+        rcases ha with ⟨ ha1,⟨p,ha2⟩,ha3⟩
+        specialize ha3 p
+        simp_all
+        rw [←ha2]
+        simp
+        assumption
+      }
+      unfold hsingle qimpl himpl
+      intro v h hh haa
+      simp [pay_index] at ha
+      rcases ha with ⟨ ha1,⟨p,ha2⟩,ha3⟩
+      specialize ha3 p
+      specialize haa ha1 p
+      simp_all only [not_true_eq_false, imp_false, not_le]
+    )
+    have eq : [∗i in ⟪0, pay_index \ {x | ∃ p ≥ 0, (default_trm, p) = x}⟫ ∪ ∅| Hx] = [∗i in {x | ∃ p < 0, ⟨0, (default_trm, p)⟩ = x}| Hx] := by
+      apply bighstar_set_eq
+      unfold labSet; rw [Set.union_empty]
+      unfold pay_index;
+      ext x
+      constructor
+      · intro ⟨x₁, ⟨⟨p, ⟨h1,h2⟩⟩, hnot⟩, hx⟩
+        simp at hnot
+        refine ⟨p, ?_, ?_⟩
+        · by_contra hge
+          have hp0 : 0 ≤ p := le_of_not_lt hge
+          have hcontra := hnot p hp0 h2
+          contradiction
+        · rw [←hx, ←h2]
+      · intro ⟨p, hp, hx⟩
+        refine ⟨(default_trm, p), ⟨⟨p, trivial, rfl⟩, ?_⟩, hx⟩
+        intro ⟨p', hp', heq⟩
+        simp [heq] at hp' hp
+        simp_all
+        exact lt_irrefl p (lt_of_lt_of_le hp hp')
+
+    rw [←eq]; clear eq
+    apply hhimpl_trans ; apply tmp
+    clear tmp
+    apply hwp_conseq
+    unfold pay_index
+    ysimp
+    unfold bighstar bighstarDef ; open Classical in simp
+    intro h hh a ha
+    specialize hh a
+    by_cases h : a.lab = 0
+    · specialize ha h
+      have hfalse :
+        ¬((a.lab = 0) ∧ (∃ p, (default_trm, p) = a.val) ∧ ∀ (x : payload), 0 ≤ x → ¬(default_trm, x) = a.val) := by
+        intro hcon
+        rcases hcon with ⟨_, ⟨p, hp⟩, hforall⟩
+        rcases ha p hp with ⟨x, hx₀, hxval⟩
+        have hcontra := hforall x hx₀
+        contradiction
+      simp [hfalse] at hh
+      assumption
+    · simp [h] at hh
+      assumption
+  }
+  -/
+  dsimp
+  /-
+  set pay_index2 : Set (trm × payload) := {x | ∃ p ≥ 0, (default_trm, p) = x} with hp2
+  have pidx_eq : {x | ∃ p ≥ 0, ⟨0, (default_trm, p)⟩ = x} = ⟪0,pay_index2⟫ := by
+    unfold labSet pay_index2
+    simp
+  rw [pidx_eq]; clear pidx_eq
+  -/
+  unfold LGTM.wp ; simp
+  have eq : (⟪0, pay_index⟫ ∪ ⟪1, lang_index⟫) =
+    ⋃ (i : payload), ({⟨0, (default_trm, i)⟩} ∪
+      {⟨1, ([lang| fun ⸨xl: Loc⸩ ⸨yl : Loc⸩=> {cfgexp_grammar i trm1 trm2}], default_payload)⟩}) := by
+    simp only [Set.iUnion_union_distrib] ; congr! 1
+    · ext a ; rcases a with ⟨al, aval⟩ ; simp [pay_index] ; aesop
+    · ext a ; rcases a with ⟨al, aval⟩ ; simp [lang_index, lang_fun_list, lang_squeeze_list] ; aesop
+  rw [← Set.biUnion_univ] at eq
+  rw [eq]
+  -- apply htriple_conseq
+  -- on_goal 2=> apply hhimpl_refl
+  apply htriple_htriple_bighstar_partition
+    (Q := fun i _ =>
+      hforall fun j =>
+      hforall fun (_ :
+      i ∈ (({⟨0, (default_trm, j)⟩} ∪
+      {⟨1, ([lang| fun ⸨xl: Loc⸩ ⸨yl : Loc⸩=> {cfgexp_grammar j trm1 trm2}], default_payload)⟩}) : Set (trm × payload)ˡ)) =>
+      (xl ~~> (xv + Int.ofNat j) ∗ yl ~~> (yv + Int.ofNat j)))
+  on_goal 1=> {
+    intro i _ j _ h
+    simp_all ; constructor
+    on_goal 2=> aesop
+    intro h1
+    dsimp [trm_funs] at h1; simp_all
+    apply cfgexp_grammar_injective (t1 := trm1) (t2 := trm2) at h1
+    aesop
+    unfold trm1; simp
+    unfold trm2; simp
+  }
+  on_goal 2=> intros ; rfl
+  { intro k _ ; dsimp only
+    have tmp := example3_single_iter (sn := trm_funs [trm_varl "xl", trm_varl "yl"] (cfgexp_grammar k trm1 trm2)) (xl := xl) (yl := yl) (n := k) (yv := yv) (xv := xv) (by rfl)
+    unfold LGTM.wp at tmp ; dsimp only [LGTM.SHTs.set, LGTM.SHTs.htrm] at tmp
+    simp only [labSet, Set.mem_singleton_iff, exists_eq_left,
+      Set.setOf_eq_eq_singleton', Set.union_empty] at tmp
+    apply htriple_conseq
+    rw [hwp_ht_eq] at tmp ; apply tmp
+    { whnf ; simp [lang_index, lang_fun_list, lang_squeeze_list, pay_index] }
+    { apply hhimpl_refl }
+    { intro hv hh hpre ; whnf at hpre ⊢ ; intro a ; specialize hpre a ; split
+      next h=>
+        simp only [h, reduceIte] at hpre
+        whnf ; intro j ; whnf ; intro h'
+        simp at h h' ; rcases h with (h | h) <;> rcases h' with (h' | h') <;> rw [h'] at h <;> simp at h
+        { simp [trm_funs] at h
+          apply cfgexp_grammar_injective at h
+          aesop
+          unfold trm1; simp
+          unfold trm2; simp
+        }
+        { aesop }
+      next h=> simp only [h, reduceIte] at hpre ; assumption
+    }
+  }
+  /-
+  apply weird_infdisj_lemma (s1 := pay_index2) (s2 := lang_index) (Hx := Hx)
+    (f := fun i => (default_trm, Int.ofNat i))
+    (g := fun i => ([lang| fun ⸨xl: Loc⸩ ⸨yl : Loc⸩ => {cfgexp_grammar i trm1 trm2}],default_payload))
+    (Idx := @Set.univ ℕ)
+  simp; simp;
+  {
+    unfold pay_index2; ext x
+    constructor <;> intro h
+    · simp_all; rcases h with ⟨p, h1,h2⟩; rw [← h2]; simp; use Int.toNat p; simp_all
+    · simp_all; rcases h with ⟨y, h1,h2⟩; use Int.toNat y; simp
+  }
+  { unfold lang_index lang_fun_list lang_squeeze_list; ext x
+    constructor <;> simp_all
+  }
+  { simp; intro i j h; rw [Prod.ext_iff] at h; simp_all }
+  { intro i j h; rw [Prod.ext_iff] at h;
+    rcases h with ⟨h1,h2⟩
+    simp_all
+    unfold trm_funs at h1; simp_all
+    unfold trm_funs at h1; simp_all
+    apply cfgexp_grammar_injective (t1 := trm1) (t2 := trm2)
+    unfold trm1; simp
+    unfold trm2; simp
+    assumption }
+  intro k hk
+  rw [hhx]
+  have pr : {⟨0, (default_trm, Int.ofNat k)⟩} = ⟪0,{(default_trm, Int.ofNat k)}⟫ := by unfold labSet; simp
+  have lr : {⟨1, (trm_funs [trm_varl "xl", trm_varl "yl"] (cfgexp_grammar k trm1 trm2), default_payload)⟩} = ⟪1, {(trm_funs [trm_varl "xl", trm_varl "yl"] (cfgexp_grammar k trm1 trm2), default_payload)}⟫ := by unfold labSet; simp
+  rw [pr,lr]; clear pr lr
+  have idx_eq : insert ⟨0, (default_trm, Int.ofNat k)⟩ ⟪1, {(trm_funs [trm_varl "xl", trm_varl "yl"] (cfgexp_grammar k trm1 trm2), default_payload)}⟫ =
+    {⟨0, (default_trm, Int.ofNat k)⟩ } ∪ {⟨1, (trm_funs [trm_varl "xl", trm_varl "yl"] (cfgexp_grammar k trm1 trm2), default_payload)⟩} := by
+    unfold labSet; aesop
+  rw [idx_eq]; clear idx_eq
+  apply example3_single_iter (sn := trm_funs [trm_varl "xl", trm_varl "yl"] (cfgexp_grammar k trm1 trm2)) (xl := xl) (yl := yl) (n := k) (yv := yv) (xv := xv)
+  simp
+  -/
