WeirdLogic/InfInfProd.lean
@@ -1,0 +1,317 @@
+import Lgtm.Hyper.ProofMode
+
+import WeirdLogic.LgtmMisc
+
+open Classical trm val prim
+
+section
+
+variable (pf : β → Set α) (s : Set β)
+  (hdj : ∀ i ∈ s, ∀ j ∈ s, i ≠ j → Disjoint (pf i) (pf j))
+
+include hdj in
+theorem fun_union_exists :
+  ∃ aux : α → Option β,
+    (∀ a i, i ∈ s ∧ a ∈ pf i ↔ aux a = some i) := by
+  have tmp := skolem (b := fun _ => Option β) (p := fun a c => ∀ (i : β), i ∈ s ∧ a ∈ pf i ↔ c = some i)
+  rw [← tmp]
+  intro a
+  by_cases h : ∃ i ∈ s, a ∈ pf i
+  · rcases h with ⟨i, iin, ain⟩
+    exists some i
+    intro v ; constructor
+    · rintro ⟨vin, ain'⟩
+      congr ; specialize hdj i iin v vin ; rw [Set.disjoint_iff_forall_ne] at hdj
+      rw [← @not_not (i = v)] ; intro c ; specialize hdj c ; apply hdj ain ain' ; rfl
+    · intro h ; simp at h ; subst_eqs ; aesop
+  · simp at h
+    exists none
+    clear tmp ; intro v ; aesop
+
+variable (Q : β → hval α → hhProp α)
+  -- this is required in some form (maybe not this strong), since
+  -- `Q v` might assert on some initial heap that can be modified by others;
+  -- if not asserted here, then the form of the post-condition in the goal
+  -- must change
+
+  -- NOTE: in this case, `Q` cannot be something like `bighstar`,
+  -- since `bighstar` asserts on the whole hyper-heap, including parts
+  -- outside `pf v`
+
+  -- `hhlocal (pf v) (Q v hv)` DOES NOT imply this
+  (hQlocal2 : ∀ v ∈ s, ∀ hv hh1 hh2, (∀ a, a ∈ pf v → hh1 a = hh2 a) → Q v hv hh1 = Q v hv hh2)
+  -- same reason as above
+  (hQlocal1 : ∀ v ∈ s, ∀ hv1 hv2, (∀ a, a ∈ pf v → hv1 a = hv2 a) → Q v hv1 = Q v hv2)
+
+include hQlocal2 hQlocal1 in
+theorem heval_heval_prod
+  (hh : β → hheap α) (ht : β → htrm α)
+  -- `aux` is to be eliminated; it is just auxiliary here
+  (aux : α → Option β)
+  :
+  -- this implies that `pf`s are disjoint
+  (∀ a i, i ∈ s ∧ a ∈ pf i ↔ aux a = some i) →
+  -- writing in this form to facilitate skolemization
+  (∀ (a : { a : β // a ∈ s }), heval (pf a) (hh a) (ht a) (Q a)) →
+  heval (⋃ i ∈ s, pf i)
+    (fun a => (aux a).elim ∅ (hh · a))
+    (fun a => (aux a).elim [lang| ()] (ht · a))
+    (fun hv => h∀ i, h∀ (_ : i ∈ s), Q i hv) := by
+  intro haux h1
+  unfold heval at h1 ; rw [skolem] at h1 ; rcases h1 with ⟨hQQ, h1⟩
+  exists (fun a v => hexists fun x => hexists fun (_ : a ∈ pf x.val) => (hQQ x a v))   -- ?
+  constructor
+  · whnf ; simp ; intro a x xin ain
+    specialize h1 ⟨_, xin⟩ ; apply And.left at h1 ; whnf at h1 ; simp at h1
+    specialize h1 _ ain
+    specialize haux a x ; simp [xin, ain] at haux ; rw [haux] ; simp
+    apply eval_conseq ; assumption
+    intro vv hh hq
+    exists ⟨x, xin⟩ ; dsimp ; exists ain
+  · intro hv h
+    unfold bighstarDef ; simp
+    intro hpre
+    exists hv ; dsimp ; whnf ; intro v ; whnf ; intro vin
+    specialize h1 ⟨_, vin⟩ ; apply And.right at h1
+    specialize h1 hv (fun a => (if a ∈ pf v then h a else hh v a))
+    unfold bighstarDef at h1 ; simp at h1
+    specialize h1 (by
+      intro a ; specialize hpre a ; split
+      next h=>
+        rw [if_pos] at hpre
+        on_goal 2=> exists v
+        rcases hpre with ⟨⟨v', v'in⟩, z, hpre⟩ ; dsimp at z
+        have haux1 := haux a v ; simp [vin, h] at haux1
+        have haux2 := haux a v' ; simp [v'in, z] at haux2
+        rw [haux1] at haux2 ; simp at haux2 ; subst v'
+        have eqproof : vin = v'in := by simp
+        rw [eqproof] ; assumption
+      next hnotin=>
+        intro ; contradiction
+    )
+    rcases h1 with ⟨hv', h1⟩
+    rw [hQlocal2 (hh2 := h)] at h1 <;> try assumption
+    on_goal 2=> simp ; intros ; contradiction
+    revert h1 ; apply Iff.mp ; rw [← propext_iff] ; apply congr_fun ; apply hQlocal1 <;> try assumption
+    intro a h ; simp ; intros ; contradiction
+
+include hdj hQlocal2 hQlocal1 in
+theorem htriple_htriple_partition
+  (hh : α → hProp) (ht : β → htrm α) (ht' : htrm α) :
+  (∀ k ∈ s, htriple (pf k) (ht k) [∗ i in (pf k)| hh i] (Q k)) →
+  (∀ i ∈ s, ∀ j ∈ pf i, ht' j = ht i j) →
+  -- `[∗ i in (⋃ j ∈ s, pf j)| hh i]` might be restrictive,
+  -- but generalizing it requires a different notation of
+  -- "big separating conjunction" over disjoint unions, so leave it for now
+  htriple (⋃ i ∈ s, pf i) ht' [∗ i in (⋃ j ∈ s, pf j)| hh i]
+    (fun hv => h∀ i, h∀ (_ : i ∈ s), Q i hv) := by
+  intro h1 hht
+  apply fun_union_exists at hdj
+  rcases hdj with ⟨aux, hdj_aux⟩
+  intro h hpre ; unfold bighstar bighstarDef at hpre ; simp at hpre
+  have tmp := heval_heval_prod pf s Q hQlocal2 hQlocal1 (fun _ => h) ht aux hdj_aux ; simp at tmp
+  have eq1 : (fun a ↦ (aux a).elim ∅ fun x ↦ h a) = h := by
+    funext a
+    rcases ho : aux a with _ | x
+    · simp ; specialize hpre a ; split at hpre
+      next hh=> rcases hh with ⟨i, hh⟩ ; rw [hdj_aux] at hh ; rw [hh] at ho ; contradiction
+      next => rw [hpre]
+    · rfl
+  rw [eq1] at tmp ; clear eq1
+  specialize tmp (by
+    intro k kin ; specialize h1 _ kin (fun a => if a ∈ pf k then h a else ∅)
+    unfold bighstar bighstarDef at h1 ; simp at h1
+    specialize h1 (by
+      intro a ; split
+      next hh=>
+        specialize hpre a ; split at hpre
+        next=> assumption
+        next hhh=> simp at hhh ; clear *- kin hh hhh ; aesop
+      next=> intros ; contradiction
+    )
+    -- well, why need to prove this?
+    whnf at h1 ⊢ ; rcases h1 with ⟨hQ', hnr, hbd⟩
+    exists hQ' ; constructor
+    · whnf at hnr ⊢ ; intro a ain ; specialize hnr _ ain ; simp [ain] at hnr ; assumption
+    · intro hv hha hpre ; unfold bighstarDef at hpre ; simp at hpre
+      specialize hbd hv (fun a => if a ∈ pf k then hha a else ∅) (by
+        simp ; intro a ; split
+        next hh=> specialize hpre a ; simp [hh] at hpre ; assumption
+        next=> rfl
+      )
+      rcases hbd with ⟨hv', hbd⟩ ; exists hv'
+      dsimp ; rw [hQlocal2] <;> (try assumption) ; intro a ain ; simp [ain]
+  )
+  rw [heval_ht_eq] ; assumption
+  whnf ; simp ; intro a b bin ain
+  specialize hdj_aux a b ; simp [ain, bin] at hdj_aux ; rw [hdj_aux] ; simp ; apply hht <;> assumption
+
+omit Q in
+include hdj in
+/-- `htriple_htriple_partition` but specialized for `bighstar` -/
+theorem htriple_htriple_bighstar_partition
+  (Q : α → val → hProp)
+  (hh : α → hProp) (ht : β → htrm α) (ht' : htrm α) :
+  (∀ k ∈ s, htriple (pf k) (ht k) [∗ i in (pf k)| hh i]
+    (fun hv => [∗ i in (pf k)| Q i (hv i) ])) →
+  (∀ i ∈ s, ∀ j ∈ pf i, ht' j = ht i j) →
+  htriple (⋃ i ∈ s, pf i) ht' [∗ i in (⋃ j ∈ s, pf j)| hh i]
+    (fun hv => [∗ i in (⋃ j ∈ s, pf j)| Q i (hv i)]) := by
+  intro h1 hht
+  let Qd : β → hval α → hhProp α := fun k hv hh => ∀ i ∈ pf k, Q i (hv i) (hh i)
+  have tmp : ∀ k ∈ s, htriple (pf k) (ht k) [∗i in pf k| hh i] (Qd k) := by
+    intro k kin ; specialize h1 k kin
+    apply htriple_conseq ; assumption ; apply hhimpl_refl
+    intro hv hh hpre ; whnf at hpre ; simp at hpre ; simp [Qd]
+    intro a ain ; specialize hpre a ; simp [ain] at hpre ; assumption
+  clear h1
+  apply htriple_htriple_partition (ht := ht) (ht' := ht') at tmp ; rotate_left
+  { assumption }
+  { intros ; simp [Qd] ; aesop }
+  { intros ; simp [Qd] ; aesop }
+  specialize tmp ‹_› ; rw [htriple_hlocal_add_to_post] at tmp
+  on_goal 2=> simp
+  apply htriple_conseq ; assumption ; apply hhimpl_refl
+  rintro hv hh ⟨hl, hpre⟩ ; simp [hhforall, Qd] at hpre ; whnf
+  intro a ; split
+  next h=> simp at h ; rcases h with ⟨k, kin, hq⟩ ; apply hpre <;> assumption
+  next => apply hl ; assumption
+
+-- is this anywhere?
+theorem triple_single_htriple (H : hProp) (Q : val → hProp) (t : trm) :
+  triple t H Q ↔
+  htriple {a} (fun _ => t) [∗ in {a} | H] (fun hv => [∗ in {a} | Q (hv a)]) := by
+  constructor
+  · intro h hh hpre ; whnf at hpre ; simp at hpre
+    have hpre' := hpre a
+    simp at hpre' ; specialize h _ hpre'
+    whnf
+    exists (fun _ => Q) ; constructor
+    · whnf ; simp ; assumption
+    · intro hv h' hpre' ; whnf at hpre' ; simp at hpre'
+      simp ; exists hv ; simp ; whnf ; simp
+      intro a' ; specialize hpre' a' ; split
+      · subst a' ; simp at hpre' ; assumption
+      · rename_i hi ; specialize hpre a' ; simp [hi] at hpre' hpre ; rw [hpre', hpre]
+  · intro h hh hpre
+    specialize h (fun a' => if a = a' then hh else ∅)
+      (by
+        whnf ; simp ; intro a' ; split
+        · subst a' ; simp ; assumption
+        · intro ; subst_eqs ; contradiction)
+    rcases h with ⟨hQ', hnr, hbd⟩
+    whnf at hnr ; unfold bighstarDef at hbd ; simp at hnr hbd
+    apply eval_conseq ; assumption
+    intro v hh hhh
+    specialize hbd (fun _ => v) (fun a' => if a = a' then hh else ∅)
+      (by
+        simp ; intro a' ; split
+        · subst a' ; simp ; assumption
+        · rename_i hi ; aesop)
+    rcases hbd with ⟨hv, hq⟩ ; whnf at hq ; simp at hq
+    specialize hq a ; simp at hq ; assumption
+
+section Replay
+
+omit pf s Q in
+private theorem htriple_prod_again {s : Set α} (H : α -> hProp) (Q : α -> val -> hProp) :
+  (∀ a ∈ s, triple (ht a) (H a) (Q a)) ->
+  htriple s ht [∗ i in s| H i] (fun hv => [∗ i in s| Q i (hv i)]) := by
+  intro h
+  apply htriple_conseq
+  rw [← htriple_hlocal_add_to_post]
+  rw [← Set.biUnion_of_singleton s]
+  apply htriple_htriple_partition (hh := H) (Q := fun k hv hhe => Q k (hv k) (hhe k))
+  · simp
+  · simp ; introv ; intro vin ; introv ; intro heq ; rw [heq]
+  · simp ; introv ; intro vin ; introv ; intro heq ; rw [heq]
+  · intro k kin ; specialize h k kin ; rw [triple_single_htriple (a := k)] at h
+    have tmp : [∗x in {k}| H k] = [∗i in {k}| H i] := by
+      funext h ; unfold bighstar bighstarDef ; simp
+      constructor <;> intro h1 a <;> specialize h1 a <;> aesop
+    rw [tmp] at h ; clear tmp
+    rw [← hwp_equiv] at h ⊢
+    rw [hwp_ht_eq (ht₂ := ht)] at h
+    apply hhimpl_trans ; apply h ; apply hwp_conseq ; intro hv hhh hpre ; whnf at hpre ; simp at hpre ; specialize hpre k ; simp at hpre ; assumption
+    whnf ; simp
+  · simp
+  · simp
+  · rw [Set.biUnion_of_singleton] ; apply hhimpl_refl
+  · rintro hv hhh ⟨hl, hpre⟩ ; whnf at hpre ⊢ ; unfold hhforall at hpre ; simp at *
+    intro a ; split ; aesop ; rw [hl] ; assumption
+
+end Replay
+
+abbrev Set.dprod (s : Set α) (pf : α → Set β) : Set (α × β) :=
+  ⋃ i ∈ s, ({i} : Set α) ×ˢ (pf i)
+
+include hQlocal2 hQlocal1 in
+theorem htriple_htriple_prod
+  (hh : β → α → hProp) (ht : β → htrm α) :
+  (∀ k ∈ s, htriple (pf k) (ht k) [∗ i in (pf k)| hh k i] (Q k)) →
+  htriple (Set.dprod s pf) (Function.uncurry ht)
+    [∗ ij in (Set.dprod s pf)| hh ij.1 ij.2]
+    (fun hv hh =>
+      ∀ i ∈ s, Q i (Function.curry hv i) (Function.curry hh i)) := by
+  intro hprod
+  -- do the injective substitution first
+  have hprod' : ∀ k ∈ s, htriple (({k} : Set β) ×ˢ (pf k)) (Function.uncurry ht)
+    [∗ ij in (({k} : Set β) ×ˢ (pf k))| hh ij.1 ij.2]
+    (fun hv hh => Q k (Function.curry hv k) (Function.curry hh k)) := by
+    intro k kin ; specialize hprod k kin
+    rw [← hwp_equiv, hwp_ht_eq (ht₂ := (ht k) ∘ Prod.snd)]
+    on_goal 2=> whnf ; simp ; intros ; subst_eqs ; rfl
+    -- CHECK the localness requirement of `htriple_hsubst`
+    rw [hwp_equiv, htriple_hlocal_add_to_post]
+    on_goal 2=> simp
+    apply htriple_hsubst
+    · whnf ; simp ; intros ; subst_eqs ; simp
+    · simp
+    · intro hv ; whnf ; simp +unfoldPartialApp [Function.curry] ; intros ; assumption
+      -- apply hQlocal2' at hq <;> try assumption
+      -- whnf at hq ⊢ ; simp at hq ⊢ ; intros
+    · rw [ssubst_image'', Set.snd_image_prod]
+      on_goal 2=> simp
+      rw [htriple_hlocal_add_to_post] at hprod
+      apply htriple_conseq ; assumption
+      · intro h hpre ; whnf at hpre ⊢ ; rcases hpre with ⟨h', heq, hpre1, hpre2⟩
+        whnf at hpre1 ; simp at hpre1
+        subst h ; intro b
+        simp ; split
+        next hin=>
+          apply fsubst_σ (x := (k, b)) at hpre2 ; simp at hpre2
+          specialize hpre1 k b ; simp [hin] at hpre1
+          simp [hin] at hpre2 ; rw [hpre2] ; assumption
+        next =>
+          rw [fsubst_out] ; rfl ; rw [ssubst_image''] ; simp ; assumption
+      · rintro hv h ⟨hl, hpre⟩
+        whnf-- ; exists (fun ij => if ij.fst = k then h ij.snd else ∅)
+        -- exists (h ∘ Prod.snd) ; split_ands
+        exists (fun ij => if ij.fst = k then h ij.snd else ∅) ; split_ands
+        · -- why this thing keeps appearing?
+          funext a ; symm
+          by_cases hin : a ∈ pf k
+          · --rw [fsubst_comp_σ] ; assumption
+            have tmp := fun f hh => fsubst_σ (@Prod.snd β α) (({k} ×ˢ pf k)) (γ := heap) (x := (k, a)) f hh (by simp ; exact hin)
+            dsimp at tmp ; rw [tmp] ; simp
+            whnf ; simp ; aesop
+          · rw [hl] <;> try assumption
+            apply fsubst_out ; simp [ssubst_image''] ; assumption
+        · whnf at hl ⊢ ; simp ; aesop
+        · simp +unfoldPartialApp [Function.curry] ; apply hpre
+        · whnf ; simp ; aesop
+      · simp
+  apply htriple_htriple_partition (α := β × α) (ht := fun _ => Function.uncurry ht)
+    (ht' := Function.uncurry ht) at hprod' ; rotate_left
+  · intros ; simp ; left ; assumption
+  · unfold Function.curry ; simp
+    intros ; rw [hQlocal2] <;> try assumption
+    rename_i hh ; intros ; apply hh <;> (solve | rfl | assumption)
+  · unfold Function.curry
+    intros ; funext hh ; rw [hQlocal1] <;> try assumption
+    rename_i hhh ; intros ; apply hhh ; simp ; assumption
+  · specialize hprod' (by intros ; rfl)
+    apply htriple_conseq ; assumption ; apply hhimpl_refl
+    intro hv h ; simp [hhforall]
+
+end
