WeirdLogic/LgtmMisc.lean
@@ -1,0 +1,344 @@
+import Lgtm.Hyper.ProofMode
+
+open Unary prim val trm
+open Classical
+
+section AddLocal
+
+-- is this anywhere?
+theorem heval_hlocal_add_to_post :
+  hlocal s h →
+  (heval s h ht hQ ↔ heval s h ht (fun hv hh => hlocal s hh ∧ hQ hv hh)) := by
+  intro hl ; constructor
+  on_goal 2=> intro h ; apply heval_conseq ; exact h ; intro hv hh ; simp
+  intro hpre
+  rcases hpre with ⟨hQ', h2a, h2b⟩
+  unfold heval
+  exists hQ'
+  constructor
+  · assumption
+  · intro hv ; specialize h2b hv
+    unfold bighstarDef at *
+    intro h_ hh_ ; specialize h2b h_ hh_
+    rcases h2b with ⟨hv1, h2b⟩
+    dsimp
+    exists hv1 ; dsimp ; constructor <;> try assumption
+    intro a hnotin ; specialize hh_ a ; simp [hnotin] at hh_ ; rw [hh_] ; aesop
+
+theorem htriple_hlocal_add_to_post :
+  hhlocal s H →
+  (htriple s ht H Q ↔ htriple s ht H (fun hv hh => hlocal s hh ∧ Q hv hh)) := by
+  intro hl ; unfold htriple
+  conv => enter [2, hh, a] ; simp [← heval_hlocal_add_to_post (hl _ a)]
+
+theorem LGTM.triple_hlocal_add_to_post :
+  hhlocal shts.set H →
+  (LGTM.triple shts H Q ↔ LGTM.triple shts H (fun hv hh => hlocal shts.set hh ∧ Q hv hh)) := by
+  intro hl ; unfold LGTM.triple LGTM.wp ; (repeat rw [hwp_equiv]) ; apply htriple_hlocal_add_to_post ; assumption
+
+end AddLocal
+
+section ssubst
+
+theorem ssubst_image' {f : α → β} {s s' : Set α} :
+  validSubst f s s' → s' ⊆ s →
+  ssubst f s s' = f '' s' := by
+  intro h hsub ; ext a ; simp [fsubst_inE _ _ h]
+  whnf at hsub ; aesop
+
+theorem ssubst_image'' {f : α → β} {s : Set α} :
+  ssubst f s s = f '' s := by apply ssubst_image' <;> simp
+
+/-- Derived from `ssubst_image'` and `ssubst_image''`. -/
+theorem ssubst_subset_change {f : α → β} {s s' : Set α} :
+  validSubst f s s' → s' ⊆ s →
+  ssubst f s s' = ssubst f s' s' := by
+  intro h hsub ; rw [ssubst_image''] ; rw [ssubst_image'] <;> assumption
+
+theorem ssubst_set_union_union {f : α → β} {s1 s2 : Set α} :
+  ssubst f (s1 ∪ s2) (s1 ∪ s2) =
+  (ssubst f s1 s1) ∪ (ssubst f s2 s2) := by ext a ; simp [fsubst_inE] ; aesop
+
+end ssubst
+
+section validSubst
+
+lemma validSubst_subset {s s' : Set α} {f : α → β} {g : α → γ} :
+  s' ⊆ s → validSubst f s s' → validSubst f s g → validSubst f s' g := by intros ; whnf at * ; aesop
+
+-- is this present anywhere? no?
+lemma validSubst_comp {s : Set α} {f : α → β} {h : β → γ} :
+  validSubst f s (h ∘ f) := by exact fun a a_1 b a_2 ↦ congrArg h
+
+-- need a version with premise/conclusion about `s'`?
+-- is this present anywhere? no?
+lemma validSubst_restricted {s s' : Set α} {f : α → β} [Inhabited γ] {h : α → γ}
+  [dec : ∀ a, Decidable (a ∈ s')] :
+  validSubst f s h →
+  validSubst f s s' →
+  s' ⊆ s →
+  validSubst f s (fun a => if a ∈ s' then h a else default) := by
+  intro hv1 hv2 hsub ; whnf ; simp
+  intro a ain b bin heq
+  have heq' := heq ; apply hv1 at heq' <;> (try assumption)
+  have heq'' := heq ; apply hv2 at heq'' <;> (try assumption)
+  simp [Set.instMembership, Set.Mem, heq', heq'']
+
+lemma validSubst_comp_restricted {s : Set α} {f : α → β} {h : β → γ} [Inhabited γ]
+  [dec : ∀ a, Decidable (a ∈ s)] :
+  validSubst f s (fun a => if a ∈ s then h (f a) else default) := by
+  apply validSubst_restricted ; apply validSubst_comp ; simp ; simp
+
+theorem validSubst_bighstar {s : Set α} {f : α → β} {H : β → hProp}
+  -- write in this way to avoid having no forward dependency
+  (inst : ∀ i ∈ s, HPropExact (H (f i))) :
+  [∗i in s| H (f i)] ==> validSubst f s := by
+  intro h hh ; whnf at hh ⊢ ; simp at *
+  intro a ain b bin heq
+  have hha := hh a ; have hhb := hh b
+  simp [ain] at hha ; simp [bin] at hhb
+  rw [← heq] at hhb
+  specialize inst a ain ; rcases inst with ⟨inst⟩
+  apply inst <;> assumption
+
+instance : HPropExact (x ~~> v) := by
+  constructor ; intro he1 he2 h1 h2 ; whnf at h1 h2 ; subst_eqs ; rfl
+
+end validSubst
+
+section fsubst
+
+/-- An alternative to `fsubst_out` requiring a different premise -/
+lemma fsubst_out' {s : Set α} {b : β} [Inhabited γ] (g : α → γ) :
+  (∀ a ∈ s, f a = b → g a = default) → fsubst f s g b = default := by
+  intro h
+  rw [fsubst, partialInvSet] ; simp
+  split <;> try rfl
+  rename_i hh ; have ⟨tmp1, tmp2⟩ := Classical.choose_spec hh
+  rw [h] <;> (try rfl) <;> assumption
+
+lemma fsubst_comp_σ_whole [Inhabited γ] (g : β → γ) :
+  (∀ x, x ∉ f '' s → g x = default) →
+  ∀ x, fsubst f s (g ∘ f) x = g x := by
+  intro h x ; by_cases hin : x ∈ f '' s
+  · apply fsubst_comp_σ ; rw [ssubst_image''] ; assumption
+  · rw [fsubst_out', h _ hin]
+    intro a ain heq ; subst x ; apply h ; assumption
+
+/-- A general form of the variants of `fsubst_σ` -/
+lemma fsubst_σ_gen {s s' : Set α} [Inhabited γ] {g : α → γ}
+  (hvfsg : validSubst f s' g)
+  (hvfss : validSubst f s s') :
+  s' ⊆ s → x ∈ s' → fsubst f s g (f x) = g x := by
+  intro hsub xin
+  unfold fsubst partialInvSet
+  simp ; have xin' := hsub xin
+  have tmp : ∃ a ∈ s, f a = f x := by exists x
+  simp [tmp]
+  have ⟨tmp1, tmp2⟩ := Classical.choose_spec tmp
+  apply hvfsg <;> try assumption
+  have ha := tmp2 ; apply hvfss at tmp2 <;> try assumption
+  simp [Set.instMembership, Set.Mem] ; aesop
+
+private lemma fsubst_σ_original {s : Set α} [Inhabited γ] (g : α → γ) :
+  validSubst f s g → x ∈ s → fsubst f s g (f x) = g x := by
+  intros ; apply fsubst_σ_gen <;> (try assumption) <;> (try simp)
+
+-- a simple derivation of `fsubst_σ_gen`
+lemma fsubst_σ_subset {s s' : Set α} [Inhabited γ] {g : α → γ}
+  (hvfsg : validSubst f s' g)
+  (hvfss : validSubst f s s') :
+  s' ⊆ s → x ∈ f '' s' → fsubst f s g x = fsubst f s' g x := by
+  intro hsub hin ; simp at hin ; rcases hin with ⟨a, hin, heq⟩ ; subst x
+  rw [fsubst_σ_gen] <;> try assumption
+  rw [fsubst_σ_gen] <;> (try assumption) <;> (try simp)
+
+lemma fsubst_comp_σ_restricted {s s' : Set α} [Inhabited γ] {g : β → γ}
+  (hvfss : validSubst f s s')
+  (hsub : s' ⊆ s)
+  [dec : ∀ a, Decidable (a ∈ s')] :
+  (∀ x, x ∉ f '' s' → g x = default) →
+  ∀ b, fsubst f s (fun a => if a ∈ s' then g (f a) else default) b = g b := by
+  intro h b
+  by_cases hin : b ∈ ssubst f s s'
+  · simp [ssubst_image' hvfss hsub] at hin
+    rcases hin with ⟨a, ain, faeq⟩ ; subst b
+    rw [fsubst_σ_gen _ hvfss] <;> try assumption
+    simp [ain] ; apply validSubst_comp_restricted
+  · -- specialize hh b ; simp [hin] at hh ; rw [hh]
+    rw [ssubst_image' hvfss hsub] at hin ; apply h at hin ; rw [hin]
+    by_cases hin' : b ∈ f '' s
+    · simp at hin' ; rcases hin' with ⟨a, hin', heq⟩ ; subst b
+      rw [fsubst_σ] <;> try assumption
+      · rw [hin] ; simp
+      · apply validSubst_restricted <;> try assumption
+        apply validSubst_comp
+    · rw [fsubst_out]
+      rw [ssubst_image''] ; assumption
+
+lemma fsubst_comp_σ_restricted_restricted {s s' : Set α} [Inhabited γ] {g : β → γ}
+  (hvfss : validSubst f s s')
+  (hsub : s' ⊆ s)
+  [dec : ∀ a, Decidable (a ∈ s')] :
+  ∀ b, fsubst f s (fun a => if a ∈ s' then g (f a) else default) b =
+    (if b ∈ f '' s' then g b else default) := by
+  intro b
+  have tmp := fsubst_comp_σ_restricted (g := fun b => if b ∈ f '' s' then g b else default) hvfss hsub
+  rw [← tmp]
+  · congr! 3 ; rename_i h ; simp [Set.mem_image_of_mem _ h]
+  · intro x hin ; simp [hin]
+
+end fsubst
+
+section hsubst
+
+set_option maxHeartbeats 800000 in
+/-- A rewritten, more general version of `hsubst_bighstar` -/
+lemma hsubst_bighstar_gen (f : α → β)
+  (s s' : Set α) (H : β → hProp) :
+  s' ⊆ s →
+  validSubst f s s' →
+  hsubst f s [∗ i in s' | H (f i)] =
+  [∗ i in ssubst f s s' | H i] := by
+  intro hsub hvs ; funext h ; simp
+  unfold bighstar bighstarDef hsubst ; dsimp
+  constructor
+  · intro hh ; whnf at hh ; rcases hh with ⟨h', heq, hh1, hh2⟩
+    subst h
+    simp [fsubst_inE _ _ hvs]
+    intro a -- ; rw [fsubst_inE] <;> try assumption
+    -- open Classical in simp
+    -- TODO simplify?
+    split
+    next h=>
+      rcases h with ⟨x, ⟨_, xin⟩, haeq⟩ ; subst a
+      specialize hh1 x ; simp [xin] at hh1
+      rw [fsubst_σ f s h' hh2 (hsub xin)] ; assumption
+    next h=>
+      simp at h
+      apply fsubst_out' ; intro y yin haeq
+      by_cases hy : y ∈ s'
+      · subst a ; specialize h _ yin hy ; contradiction
+      · specialize hh1 y ; simp [hy] at hh1 ; assumption
+  · intro hh ; dsimp
+    -- exists (h ∘ f) ; split_ands
+    -- exists (fun a => if a ∈ s then (h (f a)) else ∅) ; split_ands
+    let target := (fun a => if a ∈ s' then (h (f a)) else ∅)
+    exists target ; split_ands
+    · unfold target
+      symm ; funext b ; apply fsubst_comp_σ_restricted hvs hsub
+      intro x hin ; specialize hh x ; simp only [ssubst_image' hvs hsub, hin, reduceIte] at hh
+      exact hh
+    · simp [target] ; intro a ; split
+      next h=> specialize hh (f a) ; simp only [ssubst_image' hvs hsub, Set.mem_image_of_mem _ h, reduceIte] at hh ; assumption
+      next h=> intro ; contradiction
+    · -- apply validSubst_local
+      unfold target ; apply validSubst_restricted <;> try assumption
+      apply validSubst_comp
+
+end hsubst
+
+section SubstRule
+
+set_option maxHeartbeats 800000 in
+/-- `hsubst_heval` without a strong premise -/
+lemma hsubst_heval_gen (s : Set α) :
+  -- this might be overly strong!!!
+  -- (∀ᵉ (a ∈ s) (a' ∉ s), f a ≠ f a') ->
+  validSubst f s hh →
+  hlocal s hh →
+  (∀ hv₁ hv₂, Set.EqOn hv₁ hv₂ s → Q hv₁ = Q hv₂) →
+  heval s hh (ht ∘ f) Q →
+  heval (ssubst f s s) (fsubst f s hh) ht (fun hv => hsubst f s (Q (hv ∘ f))) := by
+  move=> vs hl Qeq /heval_strongest' ![hev himp]
+  shave vsP: validSubst f s (hsP hh (ht ∘ f))
+  { move; simp [hsP]=> ???? /[dup] /vs->// }
+  -- ?
+  exists fsubst f s (hsP hh (ht ∘ f))=> ⟨b/fsubst_inE //==![a ain <-]|⟩
+  { sby srw ?fsubst_σ }
+  move=> hv h hP
+  specialize himp (hv ∘ f) (fun a => if a ∈ s then h (f a) else ∅) ?_
+  { move=> a--; move: (hP (f a))
+    simp ; split
+    next h=>
+      specialize hP (f a) ; simp only [ssubst_image'', Set.mem_image_of_mem _ h] at hP
+      simp at hP ; rw [fsubst_σ] at hP <;> assumption
+    next => rw [hl] ; assumption
+  }
+  scase: himp=> hv' /= QP
+  exists fsubst f s hv'=> /=
+  exists (fun a => if a ∈ s then h (f a) else ∅) ; split_ands
+  { funext b
+    by_cases hin : b ∈ ssubst f s s
+    · rw [ssubst_image''] at hin ; simp at hin ; rcases hin with ⟨a, ain, faeq⟩ ; subst b
+      rw [fsubst_σ] ; simp [ain]
+      · whnf ; simp ; clear *- ; aesop
+      · assumption
+    · whnf at hP ; specialize hP b ; simp [hin] at hP ; rw [hP]
+      (repeat rw [fsubst_out]) <;> try assumption
+  }
+  { rw [Qeq] ; assumption
+    whnf ; intro x xin ; simp [fsubst_in _ _ xin, xin] }
+  { whnf ; simp ; clear *- ; aesop }
+
+/-- `hsubst_htriple` without a strong premise -/
+lemma hsubst_htriple_gen (ht : htrm β) (H : hhProp α) (Q : hval α → hhProp α) (f : α → β) :
+  hhlocal s H →
+  (∀ hv₁ hv₂, Set.EqOn hv₁ hv₂ s → Q hv₁ = Q hv₂) →
+  htriple s (ht ∘ f) H Q →
+  htriple (ssubst f s s) ht (hsubst f s H) (fun hv => hsubst f s (Q (hv ∘ f))) := by
+  move=> Hl Ql htr hh ![hh -> ??]; apply hsubst_heval_gen=>//
+
+end SubstRule
+
+section DerivedRules
+
+-- relying on `hwpgen_seq`
+theorem htriple_seq :
+  htriple s ht1 H (fun _ => Q) →
+  htriple s ht2 Q QQ →
+  htriple s (fun a => trm_seq (ht1 a) (ht2 a)) H QQ := by intro h1 h2 ; ywp ; yapp h1
+
+theorem LGTM.triple_seq (shts : LGTM.SHTs α) (ht_list1 ht_list2 : List (htrm α)) :
+  List.Forall₂ (fun sht (ht1, ht2) => ∀ a ∈ sht.s, sht.ht a = trm_seq (ht1 a) (ht2 a))
+    shts (List.zip ht_list1 ht_list2) →
+  LGTM.triple (shts.zipWith (fun sht ht1 => ⟨sht.s, ht1⟩) ht_list1) H (fun _ => Q) →
+  LGTM.triple (shts.zipWith (fun sht ht2 => ⟨sht.s, ht2⟩) ht_list2) Q QQ →
+  LGTM.triple shts H QQ := by
+  intro h h1 h2
+  unfold LGTM.triple LGTM.wp
+  rw [hwp_ht_eq (ht₂ := fun a =>
+    trm_seq
+      (LGTM.SHTs.htrm (shts.zipWith (fun sht ht1 => ⟨sht.s, ht1⟩) ht_list1) a)
+      (LGTM.SHTs.htrm (shts.zipWith (fun sht ht2 => ⟨sht.s, ht2⟩) ht_list2) a))]
+  on_goal 2=>
+    whnf ; intro x hin ; dsimp ; clear h1 h2
+    generalize he : (ht_list1.zip ht_list2) = l at h
+    induction h generalizing ht_list1 ht_list2 with
+    | nil => simp at hin ⊢
+    | @cons a b shts' l' hr hsub ih =>
+      rcases a with ⟨s, ht⟩ ; rcases b with ⟨ht1, ht2⟩
+      dsimp at hr
+      rw [List.zip_eq_cons_iff] at he ; rcases he with ⟨ht_list1', ht_list2', hh1, hh2, hl'⟩
+      subst ht_list1 ht_list2 l' ; dsimp
+      split <;> aesop
+  apply List.Forall₂.length_eq at h ; simp at h
+  have hs1 :
+    (LGTM.SHTs.set (shts.zipWith (fun sht ht1 => ⟨sht.s, ht1⟩) ht_list1)) = shts.set := by
+    have h' : shts.length ≤ ht_list1.length := by omega
+    clear *- h' ; induction shts generalizing ht_list1 with
+    | nil => simp
+    | cons sht shts' ih =>
+      rcases ht_list1 with _ | ⟨ht1, ht_list1'⟩ <;> simp at h' ; simp [ih _ h']
+  have hs2 :
+    (LGTM.SHTs.set (shts.zipWith (fun sht ht2 => ⟨sht.s, ht2⟩) ht_list2)) = shts.set := by
+    have h' : shts.length ≤ ht_list2.length := by omega
+    clear *- h' ; induction shts generalizing ht_list2 with
+    | nil => simp
+    | cons sht shts' ih =>
+      rcases ht_list2 with _ | ⟨ht2, ht_list2'⟩ <;> simp at h' ; simp [ih _ h']
+  apply htriple_seq
+  · rw [← hs1] ; exact h1
+  · rw [← hs2] ; exact h2
+
+end DerivedRules
