WeirdLogic/WLogic.lean
@@ -1,6 +1,7 @@
 import WeirdLogic.Gram
 import WeirdLogic.WTriple
 import WeirdLogic.WUtil
+import WeirdLogic.InfInfProd
 
 import Lgtm.Common.Util
 
@@ -442,27 +443,6 @@ lemma weird_grmdisj_lemma_safe_clean (s' s : Set (α × β)) (sht_prog sht_lang 
   }
   { exact pre}
 
-
-theorem tmp1 :
-  hhlocal shts.set H₁ ->
-  H₁ ==> LGTM.wp shts Q ->
-  H₁ ==> LGTM.wp shts (fun hv hh => hlocal shts.set hh ∧ Q hv hh) := by
-  intro h1 h2 h hh ; specialize h2 _ hh ; specialize h1 _ hh
-  unfold hlocal at h1
-  unfold LGTM.wp hwp at *
-  rcases h2 with ⟨hQ', h2a, h2b⟩
-  unfold heval
-  exists hQ'
-  constructor
-  · assumption
-  · intro hv ; specialize h2b hv
-    unfold bighstarDef at *
-    intro h_ hh_ ; specialize h2b h_ hh_
-    rcases h2b with ⟨hv1, h2b⟩
-    dsimp
-    exists hv1 ; dsimp ; constructor <;> try assumption
-    intro a hnotin ; specialize hh_ a ; simp [hnotin] at hh_ ; rw [hh_] ; apply h1 ; assumption
-
 /- remove hlocal in the postcondition -/
 /- Q = fun s1 s2 => ∀ ... -/
 set_option maxHeartbeats 1600000 in
@@ -482,8 +462,9 @@ lemma weird_grmdisj_lemma_safe (s' s : Set (α × β))  (sht_prog sht_lang : LGT
   H₁ ∗ H₂ ==> LGTM.wp [sht_prog, sht_lang]
     (fun _ h => ∀ ll ∈ s, ∃ pp, pp ∈ s' ∧ h ⟨1, ll ⟩= h ⟨0, pp⟩) := by
   move=> prog lang subs sp1 sp2 sp3 sp4 hlo up1 hva up2
-  apply tmp1 at up1 ; dsimp [LGTM.SHTs.set] at up1 ; simp only [Set.union_empty] at up1
+  rw [← LGTM.triple.eq_1, LGTM.triple_hlocal_add_to_post] at up1
   on_goal 2=> dsimp [LGTM.SHTs.set] ; simp only [Set.union_empty] ; assumption
+  dsimp [LGTM.triple, LGTM.SHTs.set] at up1 ; simp only [Set.union_empty] at up1
   have subsht : LGTM.wp [sht_prog, sht_lang] (fun _ h => ∀ ll ∈ s, ∃ pp, pp ∈ s' ∧ h ⟨1, ll ⟩= h ⟨0, pp⟩) = LGTM.wp ([⟨⟪ 0, s'1⟫, sht_prog.ht ⟩, ⟨⟪ 1, s1⟫, sht_lang.ht ⟩ ] ++ [⟨⟪ 0, s'2⟫, sht_prog.ht ⟩, ⟨⟪ 1, s2⟫, sht_lang.ht ⟩]) (fun v h => ∀ ll ∈ s, ∃ pp, pp ∈ s' ∧ h ⟨1, ll ⟩= h ⟨0, pp⟩):= by
     unfold LGTM.wp
     simp
@@ -875,147 +856,6 @@ lemma weird_fix_payload2 (dt : trm) (pv : ℤ) (prog : trm):
 --   move=> hev; exists hQ=> ⟨|hv ⟩ //
 --   sby apply (hhimpl_hhexists_r hv); srw fun_insert_ff
 
-lemma heval_prod''_aux (pf : β → Set α) (s : Set β) :
-  (∀ i ∈ s, ∀ j ∈ s, i ≠ j → Disjoint (pf i) (pf j)) →
-  ∃ aux : α → Option β,
-    (∀ a i, i ∈ s ∧ a ∈ pf i ↔ aux a = some i) := by
-  intro hdj
-  have tmp := skolem (b := fun _ => Option β) (p := fun a c => ∀ (i : β), i ∈ s ∧ a ∈ pf i ↔ c = some i)
-  rw [← tmp]
-  intro a
-  by_cases h : ∃ i ∈ s, a ∈ pf i
-  · rcases h with ⟨i, iin, ain⟩
-    exists some i
-    intro v ; constructor
-    · rintro ⟨vin, ain'⟩
-      congr ; specialize hdj i iin v vin ; rw [Set.disjoint_iff_forall_ne] at hdj
-      rw [← @not_not (i = v)] ; intro c ; specialize hdj c ; apply hdj ain ain' ; rfl
-    · intro h ; simp at h ; subst_eqs ; aesop
-  · simp at h
-    exists none
-    clear tmp ; intro v ; aesop
-
-lemma heval_prod'' (hQ : β → hval α → hhProp α)
-  (pf : β → Set α) (s : Set β) (hh : β → hheap α) (ht : β → htrm α)
-  (aux : α → Option β)
-  -- this is required in some form (maybe not this strong), since
-  -- `hQ v` might assert on some initial heap that can be modified by others;
-  -- if not asserted here, then the form of the post-condition in the goal
-  -- must change
-  (hQlocal2 : ∀ v hv hh1 hh2, (∀ a, a ∈ pf v → hh1 a = hh2 a) → hQ v hv hh1 = hQ v hv hh2)
-  -- same reason as above
-  (hQlocal1 : ∀ v hv1 hv2, (∀ a, a ∈ pf v → hv1 a = hv2 a) → hQ v hv1 = hQ v hv2)
-   :
-  -- (∀ i ∈ s, ∀ j ∈ s, i ≠ j → Disjoint (pf i) (pf j)) →
-  (∀ a i, i ∈ s ∧ a ∈ pf i ↔ aux a = some i) →
-  (∀ (a : { a : β // a ∈ s }), heval (pf a) (hh a) (ht a) (hQ a)) →
-  heval (⋃ i ∈ s, pf i)
-    -- (fun a => open Classical in
-    --   if h : ∃ i ∈ s, a ∈ pf i then
-    --     hh (choose h) a
-    --   else ∅)
-    (fun a => (aux a).elim ∅ (hh · a))
-    -- (fun a => open Classical in
-    --   if h : ∃ i ∈ s, a ∈ pf i then
-    --     ht (choose h) a
-    --   else [lang| ()])
-    (fun a => (aux a).elim [lang| ()] (ht · a))
-    (fun hv => h∀ i, h∀ (_ : i ∈ s),
-      hQ i hv
-      -- ∃ʰ hv', hQ i (hv ∪_(pf i) hv')
-      ) := by
-  intro haux h1
-  unfold heval at h1 ; rw [skolem] at h1 ; rcases h1 with ⟨hQQ, h1⟩
-  exists (fun a v => hexists fun x => hexists fun (_ : a ∈ pf x.val) => (hQQ x a v))   -- ?
-  constructor
-  · whnf ; simp ; intro a x xin ain
-    specialize h1 ⟨_, xin⟩ ; apply And.left at h1 ; whnf at h1 ; simp at h1
-    specialize h1 _ ain
-    specialize haux a x ; simp [xin, ain] at haux ; rw [haux] ; simp
-    apply eval_conseq ; assumption
-    intro vv hh hq
-    exists ⟨x, xin⟩ ; dsimp ; exists ain
-  · intro hv h
-    unfold bighstarDef ; open Classical in simp
-    intro hpre
-    exists hv ; dsimp ; whnf ; intro v ; whnf ; intro vin
-    specialize h1 ⟨_, vin⟩ ; apply And.right at h1
-    specialize h1 hv (fun a => open Classical in (if a ∈ pf v then h a else hh v a))
-    unfold bighstarDef at h1 ; simp at h1
-    specialize h1 (by
-      intro a ; specialize hpre a ; split
-      next h=>
-        rw [if_pos] at hpre
-        on_goal 2=> exists v
-        rcases hpre with ⟨⟨v', v'in⟩, z, hpre⟩ ; dsimp at z
-        have haux1 := haux a v ; simp [vin, h] at haux1
-        have haux2 := haux a v' ; simp [v'in, z] at haux2
-        rw [haux1] at haux2 ; simp at haux2 ; subst v'
-        have eqproof : vin = v'in := by simp
-        rw [eqproof] ; assumption
-      next hnotin=>
-        intro ; contradiction
-    )
-    rcases h1 with ⟨hv', h1⟩
-    open Classical in rw [hQlocal2 (hh2 := h)] at h1
-    on_goal 2=> simp ; intros ; contradiction
-    revert h1 ; apply Iff.mp ; rw [← propext_iff] ; apply congr_fun ; apply hQlocal1
-    intro a h ; simp ; intros ; contradiction
-
-lemma htriple_htriple_partition
-  (pf : β → Set α) (s : Set β) (hh : α → hProp) (ht : htrm α)
-  (Q : β → hval α → hhProp α)
-  (hQlocal2 : ∀ v hv hh1 hh2, (∀ a, a ∈ pf v → hh1 a = hh2 a) → Q v hv hh1 = Q v hv hh2)
-  (hQlocal1 : ∀ v hv1 hv2, (∀ a, a ∈ pf v → hv1 a = hv2 a) → Q v hv1 = Q v hv2)
-  :
-  (∀ i ∈ s, ∀ j ∈ s, i ≠ j → Disjoint (pf i) (pf j)) →
-  (∀ k ∈ s, htriple (pf k) ht [∗ i in (pf k)| hh i] (Q k)) →
-  htriple (⋃ i ∈ s, pf i) ht [∗ i in (⋃ j ∈ s, pf j)| hh i]
-    (fun hv => h∀ i, h∀ (_ : i ∈ s), Q i hv)
-    -- (fun hv hh => ∀ i : ℕ, Q i hh)
-    := by
-  intro hdj h1
-  apply heval_prod''_aux at hdj
-  rcases hdj with ⟨aux, hdj_aux⟩
-  intro h hpre ; unfold bighstar bighstarDef at hpre ; open Classical in simp at hpre
-  have tmp := heval_prod'' (hQ := Q) pf s (fun _ => h) (fun _ => ht) aux
-    hQlocal2 hQlocal1 hdj_aux ; simp at tmp
-  have eq1 : (fun a ↦ (aux a).elim ∅ fun x ↦ h a) = h := by
-    funext a
-    rcases ho : aux a with _ | x
-    · simp ; specialize hpre a ; split at hpre
-      next hh=> rcases hh with ⟨i, hh⟩ ; rw [hdj_aux] at hh ; rw [hh] at ho ; contradiction
-      next => rw [hpre]
-    · rfl
-  rw [eq1] at tmp ; clear eq1
-  specialize tmp (by
-    intro k kin ; specialize h1 _ kin (fun a => open Classical in if a ∈ pf k then h a else ∅)
-    unfold bighstar bighstarDef at h1 ; open Classical in simp at h1
-    specialize h1 (by
-      intro a ; split
-      next hh=>
-        specialize hpre a ; split at hpre
-        next=> assumption
-        next hhh=> simp at hhh ; clear *- kin hh hhh ; aesop
-      next=> intros ; contradiction
-    )
-    -- well, why need to prove this?
-    whnf at h1 ⊢ ; rcases h1 with ⟨hQ', hnr, hbd⟩
-    exists hQ' ; constructor
-    · whnf at hnr ⊢ ; intro a ain ; specialize hnr _ ain ; simp [ain] at hnr ; assumption
-    · intro hv hha hpre ; unfold bighstarDef at hpre ; simp at hpre
-      specialize hbd hv (fun a => open Classical in if a ∈ pf k then hha a else ∅) (by
-        simp ; intro a ; split
-        next hh=> specialize hpre a ; simp [hh] at hpre ; assumption
-        next=> rfl
-      )
-      rcases hbd with ⟨hv', hbd⟩ ; exists hv'
-      dsimp ; rw [hQlocal2] ; assumption ; intro a ain ; simp [ain]
-  )
-  rw [heval_ht_eq] ; assumption
-  whnf ; simp ; intro a b bin ain
-  specialize hdj_aux a b ; simp [ain, bin] at hdj_aux ; rw [hdj_aux] ; simp
-
 /-
 lemma htriple_htriple_partition (s : Set α) (idxx : Set ℕ) (pf : ℕ -> Set α) (H : α -> hProp) (Q : ℕ -> hheap α -> Prop) :
   s = (⋃ i ∈ idxx, (pf i) ) ->
@@ -1076,18 +916,21 @@ lemma weird_infdisj_lemma (s1 s2 : Set (α × β)) (Idx : Set ℕ) (sht_prog sht
   have tmp := htriple_htriple_partition
       (α := (α × β)ˡ) (s := Idx)
       (pf := fun i => {⟨0, f i⟩, ⟨1, g i⟩ })
-      (ht := sht_prog.ht ∪_⟪0, s1⟫ sht_lang.ht ∪_⟪1, s2⟫ fun x => [lang| ()])
+      (ht := fun _ => sht_prog.ht ∪_⟪0, s1⟫ sht_lang.ht ∪_⟪1, s2⟫ fun x => [lang| ()])
+      (ht' := sht_prog.ht ∪_⟪0, s1⟫ sht_lang.ht ∪_⟪1, s2⟫ fun x => [lang| ()])
       (hh := fun i => Hx)
       (Q := fun i _ => fun h => (h ⟨1, g i⟩ )= (h ⟨0, f i⟩ )
           -- else  h ⟨1, g i⟩ = ∅ ∧ h ⟨0, f i⟩ = ∅
           )
-  specialize tmp ( by simp ; clear *- ; aesop ) (by intros ; rfl)
+  specialize tmp --( by simp ; clear *- ; aesop ) (by intros ; rfl)
     (by
       intro i hi j hj ijneq ; rw [Set.disjoint_iff_forall_ne] ; simp
       constructor <;> intro hh
       · apply injf at hh ; contradiction
       · apply injg at hh ; contradiction
     )
+    (by simp ; clear *- ; aesop )
+    (by intros ; rfl)
     (by
       intro k kin ; specialize pre k kin
       rewrite (occs := .pos [2]) [Set.pair_comm] at pre
@@ -1100,6 +943,7 @@ lemma weird_infdisj_lemma (s1 s2 : Set (α × β)) (Idx : Set ℕ) (sht_prog sht
         · have hfk : g k ∈ s2 := by rw [hg];simp; use k;
           simp [hfk]
       assumption )
+    (by intros ; rfl)
   unfold LGTM.wp
   simp [LGTM.SHTs.set, prog, lang]
   have eq : (⟪0, s1⟫ ∪ ⟪1, s2⟫) = (⋃ j ∈ Idx, {⟨0, f j⟩, ⟨1, g j⟩}) := by
